theories/Stlc/Symbolic/Free.v
@@ -42,7 +42,7 @@ From Em Require Import
   Stlc.Unification
   Stlc.Worlds.
 
-Import ctx.notations.
+Import world.notations.
 Import World.notations.
 
 Set Implicit Arguments.
@@ -70,12 +70,12 @@ Section Bind.
       end.
 End Bind.
 
-Definition assert : ⊢ʷ Ṫy -> Ṫy -> Free Unit :=
+Definition assert : ⊧ Ṫy ̂→ Ṫy ̂→ Free Unit :=
   fun w t1 t2 => Assertk t1 t2 (Ret tt).
-Definition choose : ⊢ʷ Free Ṫy :=
+Definition choose : ⊧ Free Ṫy :=
   fun w =>
-    let α := ctx.length w in
-    Choosek α (Ret (ṫy.var ctx.in_zero)).
+    let α := world.fresh w in
+    Choosek α (Ret (ṫy.var world.in_zero)).
 #[global] Arguments choose {w}.
 
 Section PrenexConversion.
@@ -83,7 +83,7 @@ Section PrenexConversion.
   Import option.notations.
 
   Definition prenex {A} :
-    ⊢ʷ Free A -> Option (Diamond alloc.acc_alloc (Prod (List (Prod Ṫy Ṫy)) A)) :=
+    ⊧ Free A ̂→ Option (Diamond alloc.acc_alloc (Prod (List (Prod Ṫy Ṫy)) A)) :=
     fix pr {w} m {struct m} :=
     match m with
     | Ret a => Some (existT w (refl, (List.nil, a)))
@@ -117,123 +117,93 @@ Section WithPredicates.
       {transΘ : Trans Θ} {lktransΘ : LkTrans Θ}
       {stepΘ : Step Θ} {lkstepΘ : LkStep Θ}.
 
-    Definition WP {A} : ⊢ʷ Free A -> Box Θ (A -> Pred) -> Pred :=
-      fix WP (w : World) (m : Free A w) (POST : Box Θ (A -> Pred) w) {struct m} :=
+    Definition WP {A} : ⊧ Free A ̂→ Box Θ (A ̂→ Pred) ̂→ Pred :=
+      fix WP (w : World) (m : Free A w) (POST : Box Θ (A ̂→ Pred) w) {struct m} :=
         match m with
         | Ret a => POST _ refl a
         | Fail => ⊥ₚ
         | Assertk t1 t2 k => t1 =ₚ t2 /\ₚ WP w k POST
         | Choosek α k =>
             Acc.wp step (WP (w ▻ α) k (fun w1 r01 => _4 POST step r01))
-            (* ∃ₚ t : Ṫy w, *)
-            (*  Ext (WP (w ▻ α) k (fun w1 r01 => _4 POST step r01)) (reduce (Θ := Sub) α t) *)
         end%P.
 
-    Definition WLP {A} : ⊢ʷ Free A -> Box Θ (A -> Pred) -> Pred :=
-      fix WLP (w : World) (m : Free A w) (POST : Box Θ (A -> Pred) w) {struct m} :=
+    Definition WLP {A} : ⊧ Free A ̂→ Box Θ (A ̂→ Pred) ̂→ Pred :=
+      fix WLP (w : World) (m : Free A w) (POST : Box Θ (A ̂→ Pred) w) {struct m} :=
         match m with
         | Ret a => POST _ refl a
         | Fail => ⊤ₚ
         | Assertk t1 t2 k => t1 =ₚ t2 ->ₚ WLP w k POST
         | Choosek α k =>
-            (* ∀ₚ t : Ty w, *)
-            (*   Ext (WLP (w ▻ α) k (fun w1 r01 => _4 POST step r01)) (reduce (R := Sub) α t) *)
             Acc.wlp step (WLP (w ▻ α) k (fun w1 r01 => _4 POST step r01))
         end%P.
 
-    Lemma wp_mono {A w0} (m : Free A w0) (P Q : Box Θ (A -> Pred) w0) :
+    Lemma wp_mono {A w0} (m : Free A w0) (P Q : Box Θ (A ̂→ Pred) w0) :
       (∀ w1 (θ : Θ w0 w1) (a : A w1), Acc.wlp θ (P w1 θ a → Q w1 θ a)) ⊢
       (WP m P -∗ WP m Q).
     Proof.
-      induction m; cbn; iIntros "#PQ".
+      induction m; cbn; iIntros "#PQ"; unfold _4.
       - iSpecialize ("PQ" $! w (refl (Refl := reflΘ)) a); auto.
         now rewrite Acc.wlp_refl wand_is_impl.
       - easy.
-      - iIntros "[#Heq HP]". iSplit; [auto|]. iRevert "HP".
-        now iApply IHm.
+      - iIntros "[#Heq HP]". iSplit; [auto|]. iRevert "HP". now iApply IHm.
       - rewrite wand_is_impl. iApply Acc.wp_mono. iModIntro.
         rewrite <- wand_is_impl. iApply IHm.
-        iIntros (w1 θ1 a1) "!>".
-        rewrite <- persist_pred_trans.
-        unfold _4.
-        rewrite persist_forall.
-        iSpecialize ("PQ" $! w1).
-        rewrite persist_forall.
-        iSpecialize ("PQ" $! (step ⊙ θ1)).
-        rewrite persist_forall.
-        iSpecialize ("PQ" $! a1).
-        Unshelve. all: eauto.
+        iIntros (w1 θ1 a1) "!>". rewrite <- persist_pred_trans.
+        rewrite persist_forall. iSpecialize ("PQ" $! w1).
+        rewrite persist_forall. iSpecialize ("PQ" $! (step ⊙ θ1)).
+        rewrite persist_forall. iSpecialize ("PQ" $! a1).
+        Unshelve. all: auto.
         now rewrite Acc.persist_wlp.
     Qed.
 
-    Lemma wlp_mono {A w0} (m : Free A w0) (P Q : Box Θ (A -> Pred) w0) :
+    Lemma wlp_mono {A w0} (m : Free A w0) (P Q : Box Θ (A ̂→ Pred) w0) :
       (∀ w1 (θ : Θ w0 w1) (a : A w1), Acc.wlp θ (P w1 θ a → Q w1 θ a)) ⊢
       (WLP m P -∗ WLP m Q).
     Proof.
-      induction m; cbn; iIntros "#PQ".
+      induction m; cbn; iIntros "#PQ"; unfold _4.
       - iSpecialize ("PQ" $! w (refl (Refl := reflΘ)) a); auto.
         now rewrite Acc.wlp_refl wand_is_impl.
       - easy.
       - iIntros "HP #Heq". rewrite <- wand_is_impl.
-        iSpecialize ("HP" with "Heq"). iRevert "HP".
-        now iApply IHm.
+        iSpecialize ("HP" with "Heq"). iRevert "HP". now iApply IHm.
       - rewrite wand_is_impl. iApply Acc.wlp_mono. iModIntro.
         rewrite <- wand_is_impl. iApply IHm.
-        iIntros (w1 θ1 a1) "!>".
-        rewrite <- persist_pred_trans.
-        unfold _4.
-        rewrite persist_forall.
-        iSpecialize ("PQ" $! w1).
-        rewrite persist_forall.
-        iSpecialize ("PQ" $! (step ⊙ θ1)).
-        rewrite persist_forall.
-        iSpecialize ("PQ" $! a1).
+        iIntros (w1 θ1 a1) "!>". rewrite <- persist_pred_trans.
+        rewrite persist_forall. iSpecialize ("PQ" $! w1).
+        rewrite persist_forall. iSpecialize ("PQ" $! (step ⊙ θ1)).
+        rewrite persist_forall. iSpecialize ("PQ" $! a1).
         Unshelve. all: eauto.
         now rewrite Acc.persist_wlp.
     Qed.
 
-    #[export] Instance proper_wp_entails {A : TYPE} {w : World} (m : Free A w):
-      Proper
-        (forall_relation
-           (fun w1 => pointwise_relation (Θ w w1)
-                        (pointwise_relation (A w1) entails)) ==>
-           entails) (@WP A w m).
+    Notation "∀ x , P" := (@forall_relation _ _ (fun x => P%signature))
+      (at level 200, x binder, right associativity) : signature_scope.
+    Notation "A → P" := (@pointwise_relation A _ P%signature) : signature_scope.
+
+    #[export] Instance proper_wp_entails {A w} (m : Free A w) :
+      Proper ((∀ w1, Θ w w1 → A w1 → entails) ==> entails) (WP m).
     Proof.
-      intros P Q PQ. unfold pointwise_relation, forall_relation in PQ.
-      iStartProof. iApply wp_mono. iIntros (w1 θ1 a1) "!>".
+      intros P Q PQ. iApply wp_mono. iIntros (w1 θ1 a1) "!>".
       rewrite <- wand_is_impl. iApply PQ.
     Qed.
 
-    #[export] Instance proper_wp_bientails {A : TYPE} {w : World} (m : Free A w):
-      Proper
-        (forall_relation
-           (fun w1 => pointwise_relation (Θ w w1)
-                        (pointwise_relation (A w1) (⊣⊢ₚ))) ==>
-           (⊣⊢ₚ)) (@WP A w m).
+    #[export] Instance proper_wp_bientails {A w} (m : Free A w) :
+      Proper ((∀ w1, Θ w w1 → A w1 → (⊣⊢ₚ)) ==> (⊣⊢ₚ)) (WP m).
     Proof.
       intros P Q PQ. unfold pointwise_relation, forall_relation in PQ.
       apply split_bientails; split; apply proper_wp_entails; intros w1 θ1 a1;
-      specialize (PQ w1 θ1 a1); now apply split_bientails in PQ.
+        specialize (PQ w1 θ1 a1); now apply split_bientails in PQ.
     Qed.
 
-    #[export] Instance proper_wlp_entails {A : TYPE} {w : World} (m : Free A w):
-      Proper
-        (forall_relation
-           (fun w1 => pointwise_relation (Θ w w1)
-                        (pointwise_relation (A w1) entails)) ==>
-           entails) (@WLP A w m).
+    #[export] Instance proper_wlp_entails {A w} (m : Free A w) :
+      Proper ((∀ w1, Θ w w1 → A w1 → entails) ==> entails) (WLP m).
     Proof.
-      intros P Q PQ. unfold pointwise_relation, forall_relation in PQ.
-      iStartProof. iApply wlp_mono. iIntros (w1 θ1 a1) "!>".
+      intros P Q PQ. iStartProof. iApply wlp_mono. iIntros (w1 θ1 a1) "!>".
       rewrite <- wand_is_impl. iApply PQ.
     Qed.
 
-    #[export] Instance proper_wlp_bientails {A : TYPE} {w : World} (m : Free A w):
-      Proper
-        (forall_relation
-           (fun w1 => pointwise_relation (Θ w w1)
-                        (pointwise_relation (A w1) (⊣⊢ₚ))) ==>
-           (⊣⊢ₚ)) (@WLP A w m).
+    #[export] Instance proper_wlp_bientails {A w} (m : Free A w):
+      Proper ((∀ w1, Θ w w1 → A w1 → (⊣⊢ₚ)) ==> (⊣⊢ₚ)) (WLP m).
     Proof.
       intros P Q PQ. unfold pointwise_relation, forall_relation in PQ.
       apply split_bientails; split; apply proper_wlp_entails; intros w1 θ1 a1;
@@ -241,14 +211,14 @@ Section WithPredicates.
     Qed.
 
     Lemma wp_bind {refltransθ : ReflTrans Θ}
-      {A B w0} (m : Free A w0) (f : Box Θ (A -> Free B) w0) :
-      forall (Q : Box Θ (B -> Pred) w0),
+      {A B w0} (m : Free A w0) (f : Box Θ (A ̂→ Free B) w0) :
+      forall (Q : Box Θ (B ̂→ Pred) w0),
         WP (bind m f) Q ⊣⊢ₚ
         WP m (fun w1 θ1 a => WP (f _ θ1 a) (_4 Q θ1)).
     Proof.
       intros. unfold _4. induction m; cbn; try (firstorder; fail).
-      - apply split_bientails; split; iApply wp_mono; iIntros (w1 θ b1) "!>";
-          rewrite trans_refl_l; auto.
+      - unfold T. apply proper_wp_bientails. intros w1 θ1 b1.
+        now rewrite trans_refl_l.
       - apply Acc.proper_wp_bientails. rewrite IHm. unfold _4.
         apply proper_wp_bientails. intros w1 θ1 a1.
         apply proper_wp_bientails. intros w2 θ2 b2.
@@ -256,54 +226,53 @@ Section WithPredicates.
     Qed.
 
     Lemma wlp_bind  {refltransθ : ReflTrans Θ}
-      {A B w1} (m : Free A w1) (f : Box Θ (A -> Free B) w1) :
-      forall (Q : Box Θ (B -> Pred) w1),
+      {A B w1} (m : Free A w1) (f : Box Θ (A ̂→ Free B) w1) :
+      forall (Q : Box Θ (B ̂→ Pred) w1),
         WLP (bind m f) Q ⊣⊢ₚ
         WLP m (fun w1 θ1 a => WLP (f _ θ1 a) (_4 Q θ1)).
     Proof.
       intros. unfold _4. induction m; cbn; try (firstorder; fail).
-      - apply split_bientails; split; iApply wlp_mono; iIntros (w1 θ b1) "!>";
-          rewrite trans_refl_l; auto.
+      - apply proper_wlp_bientails. intros w1 θ1 b1.
+        now rewrite trans_refl_l.
       - apply Acc.proper_wlp_bientails. rewrite IHm. unfold _4.
         apply proper_wlp_bientails. intros w1 θ1 a1.
         apply proper_wlp_bientails. intros w2 θ2 b2.
         now rewrite trans_assoc.
     Qed.
 
-    Lemma wp_impl {A w} (m : Free A w) (P : Box Θ (A -> Pred) w) (Q : Pred w) :
+    Lemma wp_impl {A w} (m : Free A w) (P : Box Θ (A ̂→ Pred) w) (Q : Pred w) :
       (WP m P ->ₚ Q) ⊣⊢ₚ WLP m (fun w1 r01 a1 => P w1 r01 a1 ->ₚ persist Q r01)%P.
     Proof.
       induction m; cbn; unfold _4, Basics.impl.
       - now rewrite persist_pred_refl.
       - apply impl_false_l.
       - rewrite impl_and. now rewrite IHm.
-      - rewrite Acc.wp_impl. apply Acc.proper_wlp_bientails. rewrite IHm. clear IHm.
+      - rewrite Acc.wp_impl. apply Acc.proper_wlp_bientails. rewrite IHm.
         apply proper_wlp_bientails. iIntros (w1 θ1 a1). now rewrite persist_pred_trans.
     Qed.
 
-    #[local] Existing Instance instpred_prod_ty.
-
-    Definition wp_prenex {A} :
-      ⊢ʷ Option (Diamond alloc.acc_alloc (List (Ṫy * Ṫy) * A)) -> Box Θ (A -> Pred) -> Pred :=
-      fun w0 o Q => wp_optiondiamond o (fun w1 θ '(C,a) => instpred C /\ₚ Q w1 (alloc.incl θ) a)%P.
-
-    Lemma prenex_correct {A w} (m : Free A w) (Q : Box Θ (A -> Pred) w) :
-      wp_prenex (prenex m) Q ⊣⊢ₚ WP m Q.
-    Proof.
-      induction m; cbn - [step].
-      - rewrite Acc.wp_refl. rewrite and_true_l. reflexivity.
-      - reflexivity.
-      - destruct (prenex m) as [(w' & r & C & a)|]; cbn.
-        + rewrite <- IHm.
-          rewrite Acc.and_wp_r.
-          apply Acc.proper_wp_bientails.
-          now rewrite persist_eq and_assoc.
-        + rewrite <- IHm. now rewrite and_false_r.
-      - destruct (prenex m) as [(w' & r & C & a)|]; cbn - [step] in *.
-        + rewrite Acc.wp_trans. apply Acc.proper_wp_step. now rewrite <- IHm.
-        + rewrite <- IHm. now rewrite Acc.wp_false.
-    Qed.
-
   End WithAcc.
+
+  #[local] Existing Instance instpred_prod_ty.
+
+  Definition wp_prenex {A} :
+    ⊧ Option (Diamond alloc.acc_alloc (List (Ṫy * Ṫy) * A)) ̂→
+      Box alloc.acc_alloc (A ̂→ Pred) ̂→ Pred :=
+    fun w0 o Q => wp_optiondiamond o (fun w1 θ '(C,a) => instpred C /\ₚ Q w1 θ a)%P.
+
+  Lemma prenex_correct {A w} (m : Free A w) (Q : Box alloc.acc_alloc (A ̂→ Pred) w) :
+    wp_prenex (prenex m) Q ⊣⊢ₚ WP m Q.
+  Proof.
+    induction m; cbn - [step].
+    - now rewrite Acc.wp_refl and_true_l.
+    - reflexivity.
+    - destruct (prenex m) as [(w' & r & C & a)|]; cbn.
+      + rewrite -IHm Acc.and_wp_r. apply Acc.proper_wp_bientails.
+        now rewrite persist_eq and_assoc.
+      + now rewrite -IHm and_false_r.
+    - destruct (prenex m) as [(w' & r & C & a)|]; cbn - [step] in *.
+      + rewrite Acc.wp_trans. apply Acc.proper_wp_step. now rewrite <- IHm.
+      + now rewrite -IHm Acc.wp_false.
+  Qed.
 
 End WithPredicates.
