theories/Stlc/Symbolic/FreeCheck.v
@@ -46,7 +46,7 @@ From Em Require Import
   Stlc.Unification
   Stlc.Worlds.
 
-Import ctx.notations.
+Import world.notations.
 Import World.notations.
 
 Set Implicit Arguments.
@@ -60,7 +60,7 @@ Section Generate.
   Import MonadNotations.
   Import World.notations.
 
-  Definition generate : Exp -> ⊢ʷ Ėnv -> Ṫy -> Free Ėxp :=
+  Definition generate : Exp -> ⊧ Ėnv ̂→ Ṫy ̂→ Free Ėxp :=
     fix gen e {w} Γ τ :=
       match e with
       | exp.var x =>
@@ -100,70 +100,22 @@ Section Generate.
       end.
 
   Definition reconstruct_free (e : Exp) :
-    ⊢ʷ Ėnv -> Free (Prod Ṫy Ėxp) :=
+    ⊧ Ėnv ̂→ Free (Prod Ṫy Ėxp) :=
     fun w G =>
       [θ1] τ  <- choose ;;
       [θ2] e' <- generate e G[θ1] τ ;;
       Ret (τ[θ2] , e').
 
   Definition reconstruct_optiondiamond (e : Exp) :
-    Option (Diamond alloc.acc_alloc (Ṫy * Sem Exp)) ctx.nil :=
+    Option (Diamond alloc.acc_alloc (Ṫy * Sem Exp)) world.nil :=
     option.bind (prenex (reconstruct_free e empty)) solveoptiondiamond.
 
-  Definition reconstruct_schematic (e : Exp) :
-    option (Schematic (Ṫy * Sem Exp)) :=
-    optiondiamond2schematic (reconstruct_optiondiamond e).
-
-  Definition reconstruct_grounded (e : Exp) :
-    option (Ty * Exp) :=
+  Definition reconstruct_grounded (e : Exp) : option (Ty * Exp) :=
     option.map
-      (fun s : Schematic _ =>
-         let (w, te) := s in
-         inst te (grounding w))
-      (reconstruct_schematic e).
+      (fun '(existT w (_ , te)) => inst te (grounding w))
+      (reconstruct_optiondiamond e).
 
 End Generate.
-
-(* Definition persist_sim_step_alloc_env := Sub.persist_sim_step (Θ := alloc.acc_alloc) (T := Ėnv). *)
-(* Definition persist_sim_step_alloc_ty := Sub.persist_sim_step (Θ := alloc.acc_alloc) (T := Ṫy). *)
-(* Definition persist_sim_step_alloc_sem {A} := Sub.persist_sim_step (Θ := alloc.acc_alloc) (T := Sem A). *)
-
-Ltac wsimpl :=
-  repeat
-    (rewrite ?persist_refl, ?persist_trans, ?persist_lift,
-      ?inst_lift, ?inst_persist, ?inst_refl, ?inst_trans,
-      ?inst_step_snoc, ?lk_trans, ?trans_refl_l, ?trans_refl_r,
-      ?persist_insert, ?lift_insert,
-
-      ?Pred.persist_tpb, ?Pred.persist_and, ?Pred.persist_eq,
-      ?Pred.eqₚ_refl, ?Pred.impl_true_l, ?Pred.and_true_r, ?Pred.and_true_l,
-      ?Pred.impl_true_r, ?Pred.impl_false_l, ?Pred.persist_impl, ?Pred.impl_and,
-      ?Pred.persist_exists, ?Pred.persist_forall, ?Pred.Acc.wlp_true, ?Pred.eq_pair,
-      ?Pred.eq_func,
-
-      (* ?ProgramLogic.eqₚ_env_cons, *)
-      (* ?ProgramLogic.equiv_true, *)
-
-      (* ?persist_sim_step_alloc_env, ?persist_sim_step_alloc_ty, (* ?persist_sim_step_alloc_sem, *) *)
-      ?ėxp.inst_var, ?ėxp.inst_true, ?ėxp.inst_false, ?ėxp.inst_ifte, ?ėxp.inst_absu, ?ėxp.inst_abst, ?ėxp.inst_app,
-      ?Sem.inst_pure, ?Sem.inst_fmap, ?Sem.inst_app, ?Sem.persist_pure, ?Sem.persist_fmap, ?Sem.persist_app in *;
-     cbn - [lk trans step thick]; auto);
-  repeat setoid_rewrite Pred.persist_exists;
-  repeat setoid_rewrite Pred.persist_forall;
-  repeat
-    match goal with
-    | |- context[@persist ?A ?I ?Θ ?w0 ?x ?w1 ?θ] =>
-        is_var x; generalize (@persist A I Θ w0 x w1 θ); clear x; intros x;
-        try (clear w0 θ)
-    | |- context[@lk ?Θ (ctx.snoc ?w0 ?α) ?w1 ?θ ?α ctx.in_zero] =>
-        is_var θ;
-        generalize (@lk Θ (ctx.snoc w0 α) w1 θ α ctx.in_zero);
-        clear θ w0; intros ?t
-    | |- context[fun w : World => Ṫy w] =>
-        change_no_check (fun w : World => Ṫy w) with Ṫy
-    | |- context[fun w : Ctx nat => Sem ?X w] =>
-        change_no_check (fun w : World => Sem X w) with (Sem X)
-    end.
 
 Section Correctness.
 
@@ -185,8 +137,8 @@ Section Correctness.
       ⊢ WLP (Θ := alloc.acc_alloc) (generate e G t) (fun w1 θ ee =>
                                    G[θ] |--ₚ e; t[θ] ~> ee).
   Proof.
-    induction e; cbn - [choose]; intros w G τ; unfold T, _4; wsimpl.
-    - destruct lookup eqn:?; wsimpl.
+    induction e; cbn - [choose]; intros w G τ; unfold T, _4; predsimpl.
+    - destruct lookup eqn:?; predsimpl.
       constructor. intros ι _; pred_unfold.
       constructor. now rewrite lookup_inst Heqo.
     - constructor. intros ι _. pred_unfold. constructor.
@@ -201,47 +153,43 @@ Section Correctness.
 
       rewrite wlp_bind. unfold _4.
       iPoseProof (IHe3 w2 G[θ1⊙θ2] τ[θ1⊙θ2]) as "-#IH3". iRevert "IH3". clear IHe3.
-      iApply (@wlp_mono alloc.acc_alloc). iIntros (w3 θ3 e3') "!> HT3". cbn.
-      wsimpl.
+      iApply (@wlp_mono alloc.acc_alloc). iIntros (w3 θ3 e3') "!> HT3".
+      predsimpl.
       iStopProof. constructor. intros ι (HT1 & HT2 & HT3).
-      pred_unfold. wsimpl. constructor; auto.
+      pred_unfold. constructor; auto.
 
-    - iIntros "!> !>".
-      rewrite wlp_bind. unfold _4. cbn.
+    - iIntros "!> !>". rewrite wlp_bind. unfold _4. cbn.
 
-      iPoseProof (IHe _ (G[step][step] ,, x∷lk step ctx.in_zero) (ṫy.var ctx.in_zero)) as "-#IH". iRevert "IH". clear IHe.
+      iPoseProof (IHe _ (G[step][step] ,, x∷lk step world.in_zero) (ṫy.var world.in_zero)) as "-#IH". iRevert "IH". clear IHe.
       iApply (@wlp_mono alloc.acc_alloc). iIntros (w1 θ1 e1').
-      iIntros "!> HT Heq1". rewrite persist_insert. wsimpl.
-      generalize (@lk alloc.acc_alloc (w ▻ @ctx.length nat w)
-                   (w ▻ @ctx.length nat w ▻ S (@ctx.length nat w))
-                   (@step alloc.acc_alloc alloc.step_alloc (w ▻ @ctx.length nat w)
-                      (S (@ctx.length nat w))) (@ctx.length nat w)
-                   (@ctx.in_zero nat (@ctx.length nat w) w))[θ1] as t1.
-      intros t1.
-      generalize (@lk alloc.acc_alloc (w ▻ @ctx.length nat w ▻ S (@ctx.length nat w)) w1 θ1
-                (S (@ctx.length nat w))
-                (@ctx.in_zero nat (S (@ctx.length nat w)) (w ▻ @ctx.length nat w))).
-      intros t2.
+      iIntros "!> HT Heq1". predsimpl. rewrite lk_step. cbn.
+      repeat
+        match goal with
+        | |- context[@lk ?Θ ?w0 ?w1 ?θ ?α ?αIn] =>
+            is_var θ;
+            generalize (@lk Θ w0 w1 θ α αIn);
+            intros ?t
+        end.
       iStopProof. constructor. intros ι [HT Heq]. pred_unfold.
-      rewrite inst_insert in HT. wsimpl. now constructor.
+      rewrite inst_insert in HT. now constructor.
     - iIntros "!>". rewrite wlp_bind. unfold _4. cbn.
-      iPoseProof (IHe _ (G[step] ,, x∷lift t (w ▻ ctx.length w)) (ṫy.var ctx.in_zero)) as "-#IH". iRevert "IH". clear IHe.
+      iPoseProof (IHe _ (G[step] ,, x∷lift t (w ▻ world.fresh w)) (ṫy.var world.in_zero)) as "-#IH". iRevert "IH". clear IHe.
       iApply (@wlp_mono alloc.acc_alloc). iIntros (w1 θ1 e1') "!> HT". cbn.
-      rewrite persist_insert. wsimpl.
-      iStopProof. constructor. intros ι HT1. pred_unfold. wsimpl.
+      rewrite persist_insert. predsimpl.
+      iStopProof. constructor. intros ι HT1. pred_unfold.
       rewrite inst_insert inst_lift in HT1. now constructor.
     - iIntros "!>". rewrite wlp_bind. unfold _4.
-      iPoseProof (IHe1 _ G[step] (ṫy.func (ṫy.var ctx.in_zero) τ[step])) as "-#IH". iRevert "IH". clear IHe1.
+      iPoseProof (IHe1 _ G[step] (ṫy.func (ṫy.var world.in_zero) τ[step])) as "-#IH". iRevert "IH". clear IHe1.
       iApply (@wlp_mono alloc.acc_alloc). iIntros (w1 r1 e1') "!> HT1".
       rewrite wlp_bind. unfold _4.
-      iPoseProof (IHe2 w1 G[step ⊙ r1] (lk r1 ctx.in_zero)) as "-#IH". iRevert "IH". clear IHe2.
+      iPoseProof (IHe2 w1 G[step ⊙ r1] (lk r1 world.in_zero)) as "-#IH". iRevert "IH". clear IHe2.
       iApply (@wlp_mono alloc.acc_alloc). iIntros (w2 r2 e2') "!> HT2". cbn.
-      wsimpl.
-      iStopProof. constructor. intros ι (HT1 & HT2). pred_unfold. wsimpl.
+      predsimpl.
+      iStopProof. constructor. intros ι (HT1 & HT2). pred_unfold.
       econstructor; eauto.
   Qed.
 
-  Definition TPB_algo : ⊢ʷ Ėnv -> Const Exp -> Ṫy -> Ėxp -> Pred :=
+  Definition TPB_algo : ⊧ Ėnv ̂→ Const Exp ̂→ Ṫy ̂→ Ėxp ̂→ Pred :=
     fun w0 G0 e t0 e0 =>
     WP (Θ := alloc.acc_alloc)
       (reconstruct_free e G0)
@@ -254,11 +202,10 @@ Section Correctness.
   Proof.
     iStartProof. rewrite wand_is_impl. rewrite wp_impl. unfold reconstruct_free.
     rewrite wlp_bind. cbn. unfold _4. iIntros "!>".
-    rewrite wlp_bind. cbn. unfold _4. wsimpl.
-    iPoseProof (@generate_sound_aux e _ G0[step] (ṫy.var ctx.in_zero)) as "-#Hsound".
+    rewrite wlp_bind. cbn. unfold _4. predsimpl.
+    iPoseProof (@generate_sound_aux e _ G0[step] (ṫy.var world.in_zero)) as "-#Hsound".
     iRevert "Hsound". iApply (@wlp_mono alloc.acc_alloc). iIntros (w1 θ1 e') "!> HT".
-    wsimpl. rewrite <- !persist_trans. wsimpl.
-    iStopProof. constructor. intros ι HT Heqt Heqe. now pred_unfold.
+    predsimpl. iStopProof. constructor. intros ι HT Heqt Heqe. now pred_unfold.
   Qed.
 
   Lemma generate_complete_aux {G e t ee} (T : G |-- e ∷ t ~> ee) :
@@ -270,7 +217,7 @@ Section Correctness.
   Proof.
     induction T as [G x t Hres|G|G|G t e1 e1' e2 e2' e3 e3' _ IH1 _ IH2 _ IH3
       |G x t1 t2 e e' _ IH|G x t1 t2 e e' _ IH|G e1 t2 e1' e2 t1 e2' _ IH1 _ IH2];
-      intros w0 G0 t0; wsimpl; unfold _4, Worlds.T.
+      intros w0 G0 t0; predsimpl; unfold _4, Worlds.T.
 
     - constructor. intros ι. unfold eqₚ. pred_unfold.
       intros _ -> ->.
@@ -288,73 +235,73 @@ Section Correctness.
       iPoseProof (eqₚ_intro (lift ty.bool w0)) as "Heqbool".
       iPoseProof (IH1 _ G0 ṫy.bool with "HeqG Heqbool") as "-#IH". clear IH1.
       iRevert "IH".
-      iApply (@wp_mono alloc.acc_alloc). iIntros (w1 r1 e1'') "!> #Heq1". wsimpl.
+      iApply (@wp_mono alloc.acc_alloc). iIntros (w1 r1 e1'') "!> #Heq1". predsimpl.
 
       rewrite wp_bind. unfold _4.
       iPoseProof (IH2 _ G0[r1] t0[r1] with "HeqG Heqt") as "-#IH". clear IH2.
       iRevert "IH".
-      iApply (@wp_mono alloc.acc_alloc). iIntros (w2 r2 e2'') "!> #Heq2". wsimpl.
+      iApply (@wp_mono alloc.acc_alloc). iIntros (w2 r2 e2'') "!> #Heq2". predsimpl.
 
       rewrite wp_bind. unfold _4.
       iPoseProof (IH3 _ G0 t0 with "HeqG Heqt") as "-#IH". clear IH3.
       iRevert "IH".
-      iApply (@wp_mono alloc.acc_alloc). iIntros (w3 r3 e3'') "!> #Heq3". wsimpl.
+      iApply (@wp_mono alloc.acc_alloc). iIntros (w3 r3 e3'') "!> #Heq3". predsimpl.
 
       iClear "Heqbool".
       iStopProof. constructor. intros ι [_ [(HeqG & Heqt & Heq1 & Heq2 & Heq3)]].
-      pred_unfold. wsimpl. now subst.
+      now pred_unfold.
 
     - iIntros "#HeqG #Heqt". cbn.
       rewrite Acc.intro_wp_step.
       iExists (lift t1 _). iIntros "!> #Heq1".
       rewrite Acc.intro_wp_step.
       iExists (lift t2 _). iIntros "!> #Heq2".
-      rewrite wp_bind. unfold _4. wsimpl.
-      iPoseProof (IH _ (G0 ,, x∷lk step ctx.in_zero) (ṫy.var ctx.in_zero)) as "IH".
-      clear IH. wsimpl.
-      rewrite <- eqₚ_insert. wsimpl.
+      rewrite wp_bind. unfold _4. predsimpl.
+      iPoseProof (IH _ (G0 ,, x∷lk step world.in_zero) (ṫy.var world.in_zero)) as "IH".
+      clear IH. predsimpl.
       iPoseProof ("IH" with "HeqG Heq1 Heq2") as "-#IH'"; iClear "IH". iRevert "IH'".
       iApply (@wp_mono alloc.acc_alloc).
-      iIntros (w1 r1 e1'') "!> #Heq3". wsimpl.
+      iIntros (w1 r1 e1'') "!> #Heq3". predsimpl.
       repeat
         match goal with
-        | |- context[@lk ?Θ (ctx.snoc ?w0 ?α) ?w1 ?θ ?α ctx.in_zero] =>
-            generalize (@lk Θ (ctx.snoc w0 α) w1 θ α ctx.in_zero);
+        | |- context[@lk ?Θ (world.snoc ?w0 ?α) ?w1 ?θ ?α world.in_zero] =>
+            generalize (@lk Θ (world.snoc w0 α) w1 θ α world.in_zero);
             intros ?t
         end.
-      wsimpl.
+      predsimpl.
       iStopProof. constructor. intros ι [_ [(HeqG & Heqt & Heq1 & Heq2 & Heq3)]].
-      pred_unfold. wsimpl. now subst.
+      now pred_unfold.
 
     - iIntros "#HeqG #Heqt". cbn.
       rewrite Acc.intro_wp_step.
-      iExists (lift t2 _). iIntros "!> #Heq1". wsimpl.
+      iExists (lift t2 _). iIntros "!> #Heq1". predsimpl.
 
       rewrite wp_bind. unfold _4.
-      iPoseProof (IH _ (G0 ,, x∷lift t1 _) (ṫy.var ctx.in_zero)) as "IH". clear IH. wsimpl.
-      rewrite <- eqₚ_insert. wsimpl.
+      iPoseProof (IH _ (G0 ,, x∷lift t1 _) (ṫy.var world.in_zero)) as "IH". clear IH.
+      predsimpl.
       iPoseProof ("IH" with "HeqG Heq1") as "-#IH'"; iClear "IH". iRevert "IH'".
       iApply (@wp_mono alloc.acc_alloc).
-      iIntros (w1 r1 e'') "!> #Heq2"; wsimpl.
+      iIntros (w1 r1 e'') "!> #Heq2"; predsimpl.
       iStopProof. constructor. intros ι [_ [(HeqG & Heqt & Heq1 & Heq2)]].
-      pred_unfold. wsimpl. now subst.
+      now pred_unfold.
 
     - iIntros "#HeqG #Heqt". cbn.
       rewrite Acc.intro_wp_step.
-      iExists (lift t1 _). iIntros "!> #Heq1". wsimpl.
-      rewrite wp_bind. unfold _4. wsimpl.
-      iPoseProof (IH1 _ G0[step] (ṫy.func (ṫy.var ctx.in_zero) t0)) as "IH"; clear IH1. wsimpl.
+      iExists (lift t1 _). iIntros "!> #Heq1". predsimpl.
+      rewrite wp_bind. unfold _4. predsimpl.
+      iPoseProof (IH1 _ G0[step] (ṫy.func (ṫy.var world.in_zero) t0)) as "IH"; clear IH1.
+      predsimpl.
       iPoseProof ("IH" with "HeqG Heq1 Heqt") as "-#IH'"; iClear "IH". iRevert "IH'".
       iApply (@wp_mono alloc.acc_alloc).
-      iIntros (w1 r1 e1'') "!> #Heq2"; wsimpl.
+      iIntros (w1 r1 e1'') "!> #Heq2"; predsimpl.
 
       rewrite wp_bind. unfold _4. cbn.
       iPoseProof (IH2 w1 G0 t with "HeqG Heq1") as "-#IH"; clear IH2. iRevert "IH".
       iApply (@wp_mono alloc.acc_alloc).
-      iIntros (w2 r2 e2'') "!> #Heq3"; wsimpl.
+      iIntros (w2 r2 e2'') "!> #Heq3"; predsimpl.
 
       iStopProof. constructor. intros ι [_ [(HeqG & Heqt & Heq1 & Heq2 & Heq3)]].
-      pred_unfold. wsimpl. now subst.
+      now pred_unfold.
   Qed.
 
   Lemma generate_complete (e : Exp) (w0 : World) (G0 : Ėnv w0) t0 e0 :
@@ -362,14 +309,14 @@ Section Correctness.
   Proof.
     iIntros "HT". unfold TPB_algo, reconstruct_free. rewrite wp_bind. cbn. unfold _4.
     rewrite Acc.intro_wp_step.
-    iExists t0. iIntros "!> Heq1". wsimpl.
+    iExists t0. iIntros "!> Heq1". predsimpl.
     rewrite wp_bind. unfold _4. cbn.
     iStopProof. constructor. intros ι [HT Heq]. pred_unfold.
-    pose proof (@generate_complete_aux _ _ _ _ HT _ G0 (ṫy.var ctx.in_zero)) as [Hcompl].
+    pose proof (@generate_complete_aux _ _ _ _ HT _ G0 (ṫy.var world.in_zero)) as [Hcompl].
     specialize (Hcompl ι (MkEmp _)). pred_unfold.
     specialize (Hcompl eq_refl Heq). revert Hcompl.
-    apply wp_mono. intros w1 θ1 e1.
-    wsimpl. intros ι1 <-. pred_unfold. wsimpl.
+    apply wp_mono. intros w1 θ1 e1. predsimpl.
+    intros ι1 <-. now pred_unfold.
   Qed.
 
   Lemma generate_correct (e : Exp) (w0 : World) (G0 : Ėnv w0) t0 e0 :
@@ -379,7 +326,7 @@ Section Correctness.
   Import (hints) Triangular.Tri.
   Import (hints) Acc.
 
-  Definition TPB_OD (e : Exp) (t : Ty) (ee : Exp) : Pred ctx.nil :=
+  Definition TPB_OD (e : Exp) (t : Ty) (ee : Exp) : Pred world.nil :=
     wp_optiondiamond (reconstruct_optiondiamond e)
       (fun w θ '(t', ee') => t' =ₚ lift t w /\ₚ ee' =ₚ lift ee w).
 
@@ -397,39 +344,14 @@ Section Correctness.
     rewrite wp_bind. unfold reconstruct_optiondiamond.
     rewrite wp_optiondiamond_bind'.
     unfold reconstruct_free. cbn.
-    rewrite wp_option_bind. unfold T, _4.
-    wsimpl.
+    rewrite wp_option_bind. unfold T, _4. predsimpl.
     rewrite <- prenex_correct.
-    generalize
-(@prenex (Prod Ṫy (Sem Exp)) (@ctx.snoc nat (@ctx.nil nat) 0)
-             (@bind alloc.acc_alloc Free
-                (@bind_freem alloc.acc_alloc alloc.refl_alloc alloc.trans_alloc
-                   alloc.step_alloc) (Sem Exp) (Prod Ṫy (Sem Exp))
-                (@ctx.snoc nat (@ctx.nil nat) 0)
-                (@generate e (@ctx.snoc nat (@ctx.nil nat) 0)
-                   (@persist Ėnv persist_env alloc.acc_alloc (@ctx.nil nat)
-                      (@empty (Ėnv (@ctx.nil nat))
-                         (@gmap_empty string string_eq_dec string_countable
-                            (Ṫy (@ctx.nil nat)))) (@ctx.snoc nat (@ctx.nil nat) 0)
-                      (@step alloc.acc_alloc alloc.step_alloc (@ctx.nil nat) 0))
-                   (@ṫy.var (@ctx.snoc nat (@ctx.nil nat) 0) 0
-                      (@ctx.in_zero nat 0 (@ctx.nil nat))))
-                (fun (w1 : Ctx nat)
-                   (θ2 : alloc.acc_alloc (@ctx.snoc nat (@ctx.nil nat) 0) w1)
-                   (e' : Sem Exp w1) =>
-                 @Ret (Prod Ṫy (Sem Exp)) w1
-                   (@pair (Ṫy w1) (Sem Exp w1)
-                      (@lk alloc.acc_alloc (@ctx.snoc nat (@ctx.nil nat) 0) w1 θ2 0
-                         (@ctx.in_zero nat 0 (@ctx.nil nat))) e')))).
-    intros m.
-    unfold wp_prenex, wp_optiondiamond. cbn.
-    unfold _4. cbn.
-    destruct m as [(w1 & θ1 & C & t' & ee')|]; cbn; [|now rewrite Acc.wp_false].
-    cbn. wsimpl.
+    destruct prenex as [(w1 & θ1 & C & t' & ee')|]; cbn; [|now rewrite Acc.wp_false].
+    unfold wp_prenex, wp_optiondiamond. predsimpl.
     rewrite wp_option_bind.
     rewrite <- solver_correct.
     destruct (solver C) as [(w2 & θ2 & [])|]; cbn.
-    - rewrite Acc.and_wp_l. wsimpl. clear.
+    - rewrite Acc.and_wp_l. predsimpl. clear.
       rewrite eqₚ_sym.
       generalize (t' =ₚ lift t w2). clear. intros P.
       rewrite eqₚ_sym.
@@ -437,15 +359,15 @@ Section Correctness.
       constructor; intros ι.
       destruct (env.view ι). cbn.
       split; intros [ι]; firstorder.
-      exists (env.snoc env.nil _ (inst (lk θ1 ctx.in_zero) (inst θ2 ι))).
+      exists (env.snoc env.nil _ (inst (lk θ1 world.in_zero) (inst θ2 ι))).
       split; auto.
       exists (inst θ2 ι). firstorder.
     - now rewrite and_false_l !Acc.wp_false.
   Qed.
 
   Definition tpb_algo (e : Exp) (t : Ty) (ee : Exp) : Prop :=
-    match reconstruct_schematic e with
-    | Some (existT w (t', ee')) =>
+    match reconstruct_optiondiamond e with
+    | Some (existT w (_ , (t', ee'))) =>
         exists ι : Assignment w, inst t' ι = t /\ inst ee' ι = ee
     | None => False
     end.
@@ -454,7 +376,7 @@ Section Correctness.
     tpb empty e t ee <-> tpb_algo e t ee.
   Proof.
     generalize (reconstruct_schematic_correct e t ee).
-    unfold TPB_OD, tpb_algo, reconstruct_schematic.
+    unfold TPB_OD, tpb_algo.
     intros [HE]. specialize (HE env.nil). pred_unfold.
     rewrite inst_empty in HE. rewrite HE. clear HE.
     destruct reconstruct_optiondiamond as [(w & θ & [t' ee'])|]; cbn; auto.
