theories/Stlc/Symbolic/FreeReconstruct.v
@@ -42,12 +42,11 @@ From Em Require Import
   Stlc.Predicates
   Stlc.Sem
   Stlc.Spec
-  Stlc.Substitution
   Stlc.Symbolic.Free
   Stlc.Unification
   Stlc.Worlds.
 
-Import ctx.notations.
+Import world.notations.
 Import World.notations.
 
 Set Implicit Arguments.
@@ -61,7 +60,11 @@ Section Generate.
   Import MonadNotations.
   Import World.notations.
 
-  Definition generate : Exp -> ⊢ʷ Ėnv -> Free (Ṫy * Ėxp) :=
+  Existing Class acc.
+  Existing Instance trans.
+  Hint Mode acc - + - : typeclass_instances.
+
+  Definition generate : Exp -> ⊧ Ėnv ̂→ Free (Ṫy * Ėxp) :=
     fix gen e {w} Γ :=
       match e with
       | exp.var x =>
@@ -72,25 +75,25 @@ Section Generate.
       | exp.true  => Ret (ṫy.bool, ėxp.true)
       | exp.false => Ret (ṫy.bool, ėxp.false)
       | exp.ifte e1 e2 e3 =>
-          [ θ1 ] '(t1,e1') <- gen e1 Γ ;;
-          [ θ2 ] '(t2,e2') <- gen e2 Γ[θ1] ;;
-          [ θ3 ] '(t3,e3') <- gen e3 Γ[θ1⊙θ2] ;;
-          [ θ4 ] _         <- assert ṫy.bool t1[θ2⊙θ3] ;;
-          [ θ5 ] _         <- assert t2[θ3⊙θ4] t3[θ4] ;;
-          Ret (t3[θ4⊙θ5], ėxp.ifte e1'[θ2⊙θ3⊙θ4⊙θ5] e2'[θ3⊙θ4⊙θ5] e3'[θ4⊙θ5])
+          [ _ ] '(t1,e1') <- gen e1 Γ ;;
+          [ _ ] '(t2,e2') <- gen e2 Γ[_] ;;
+          [ _ ] '(t3,e3') <- gen e3 Γ[_] ;;
+          [ _ ] _         <- assert ṫy.bool t1[_] ;;
+          [ _ ] _         <- assert t2[_] t3[_] ;;
+          Ret (t3[_], ėxp.ifte e1'[_] e2'[_] e3'[_])
       | exp.absu x e =>
-          [ θ1 ] t1       <- choose ;;
-          [ θ2 ] '(t2,e') <- gen e (Γ[θ1] ,, x∷t1) ;;
-          Ret (ṫy.func t1[θ2] t2, ėxp.abst x t1[θ2] e')
+          [ _ ] t1       <- choose ;;
+          [ _ ] '(t2,e') <- gen e (Γ[_] ,, x∷t1) ;;
+          Ret (ṫy.func t1[_] t2, ėxp.abst x t1[_] e')
       | exp.abst x t1 e =>
-          [ θ1 ] '(t2,e') <- gen e (Γ ,, x∷lift t1 _) ;;
+          [ _ ] '(t2,e') <- gen e (Γ ,, x∷lift t1 _) ;;
           Ret (ṫy.func (lift t1 _) t2, ėxp.abst x (lift t1 _) e')
       | exp.app e1 e2 =>
-          [ θ1 ] '(tf, e1') <- gen e1 Γ ;;
-          [ θ2 ] '(t1, e2') <- gen e2 Γ[θ1] ;;
-          [ θ3 ] t2 <- choose ;;
-          [ θ4 ] _  <- assert tf[θ2⊙θ3] (ṫy.func t1[θ3] t2) ;;
-          Ret (t2[θ4], ėxp.app e1'[θ2⊙θ3⊙θ4] e2'[θ3⊙θ4])
+          [ _ ] '(tf, e1') <- gen e1 Γ ;;
+          [ _ ] '(t1, e2') <- gen e2 Γ[_] ;;
+          [ _ ] t2 <- choose ;;
+          [ _ ] _  <- assert tf[_] (ṫy.func t1[_] t2) ;;
+          Ret (t2[_], ėxp.app e1'[_] e2'[_])
       end.
 
 End Generate.
@@ -98,68 +101,19 @@ End Generate.
 Section Reconstruct.
 
   Definition reconstruct_optiondiamond (e : Exp) :
-    Option (Diamond alloc.acc_alloc (Ṫy * Sem Exp)) ctx.nil :=
+    Option (Diamond alloc.acc_alloc (Ṫy * Sem Exp)) world.nil :=
     option.bind (prenex (generate e ∅)) solveoptiondiamond.
 
-  Definition reconstruct_schematic (e : Exp) :
-    option (Schematic (Ṫy * Sem Exp)) :=
-    optiondiamond2schematic (reconstruct_optiondiamond e).
-
-  Definition reconstruct_grounded (e : Exp) :
-    option (Ty * Exp) :=
+  Definition reconstruct_grounded (e : Exp) : option (Ty * Exp) :=
     option.map
-      (fun s : Schematic _ =>
-         let (w, te) := s in
-         inst te (grounding w))
-      (reconstruct_schematic e).
+      (fun '(existT w (_ , te)) => inst te (grounding w))
+      (reconstruct_optiondiamond e).
 
 End Reconstruct.
-
-Definition persist_sim_step_alloc_env := Sub.persist_sim_step (Θ := alloc.acc_alloc) (T := Ėnv).
-Definition persist_sim_step_alloc_ty := Sub.persist_sim_step (Θ := alloc.acc_alloc) (T := Ṫy).
-(* Definition persist_sim_step_alloc_sem {A} := Sub.persist_sim_step (Θ := alloc.acc_alloc) (T := Sem A). *)
-
-Ltac wsimpl :=
-  repeat
-    (rewrite ?persist_refl, ?persist_trans, ?persist_lift,
-      ?inst_lift, ?inst_persist, ?inst_refl, ?inst_trans,
-      ?inst_step_snoc, ?lk_trans, ?trans_refl_l, ?trans_refl_r,
-      ?persist_insert, ?lift_insert,
-
-      ?Pred.persist_tpb, ?Pred.persist_and, ?Pred.persist_eq,
-      ?Pred.eqₚ_refl, ?Pred.impl_true_l, ?Pred.and_true_r, ?Pred.and_true_l,
-      ?Pred.impl_true_r, ?Pred.impl_false_l, ?Pred.persist_impl, ?Pred.impl_and,
-      ?Pred.persist_exists, ?Pred.persist_forall, ?Pred.Acc.wlp_true, ?Pred.eq_pair,
-      ?Pred.eq_func,
-
-      (* ?ProgramLogic.eqₚ_env_cons, *)
-      (* ?ProgramLogic.equiv_true, *)
-
-      ?persist_sim_step_alloc_env, ?persist_sim_step_alloc_ty, (* ?persist_sim_step_alloc_sem, *)
-      ?ėxp.inst_var, ?ėxp.inst_true, ?ėxp.inst_false, ?ėxp.inst_ifte, ?ėxp.inst_absu, ?ėxp.inst_abst, ?ėxp.inst_app,
-      ?Sem.inst_pure, ?Sem.inst_fmap, ?Sem.inst_app, ?Sem.persist_pure, ?Sem.persist_fmap, ?Sem.persist_app in *;
-     cbn - [lk trans step thick Sub.up1]; auto);
-  repeat setoid_rewrite Pred.persist_exists;
-  repeat setoid_rewrite Pred.persist_forall;
-  repeat
-    match goal with
-    | |- context[@persist ?A ?I ?Θ ?w0 ?x ?w1 ?θ] =>
-        is_var x; generalize (@persist A I Θ w0 x w1 θ); clear x; intros x;
-        try (clear w0 θ)
-    | |- context[@lk ?Θ (ctx.snoc ?w0 ?α) ?w1 ?θ ?α ctx.in_zero] =>
-        is_var θ;
-        generalize (@lk Θ (ctx.snoc w0 α) w1 θ α ctx.in_zero);
-        clear θ w0; intros ?t
-    | |- context[fun w : World => Ṫy w] =>
-        change_no_check (fun w : World => Ṫy w) with Ṫy
-    | |- context[fun w : Ctx nat => Sem ?X w] =>
-        change_no_check (fun w : World => Sem X w) with (Sem X)
-    end.
 
 Section Correctness.
 
   Import Pred Pred.notations.
-  Import (hints) Sub.
   Import Pred.proofmode.
   Import iris.proofmode.tactics.
   Open Scope pred_scope.
@@ -172,24 +126,29 @@ Section Correctness.
   #[local] Arguments step : simpl never.
   (* #[local] Arguments Free.choose : simpl never. *)
 
-  Definition TPB_algo : ⊢ʷ Ėnv -> Const Exp -> Ṫy -> Ėxp -> Pred :=
+  Definition TPB_algo : ⊧ Ėnv ̂→ Const Exp ̂→ Ṫy ̂→ Ėxp ̂→ Pred :=
     fun w0 G0 e t0 e0 =>
     WP (Θ := alloc.acc_alloc)
       (generate e G0)
       (fun w1 (θ1 : alloc.acc_alloc w0 w1) '(t1,e1) =>
          t0[θ1] =ₚ t1 /\ₚ e0[θ1] =ₚ e1).
 
+  Create HintDb psimpl.
+  #[local] Hint Rewrite @inst_refl @inst_insert @inst_lift : psimpl.
+
+  Ltac psimplnew :=
+    autorewrite with psimpl in *; auto with typeclass_instances.
+
   Lemma generate_sound_aux e :
     forall (w : World) (G : Ėnv w),
       ⊢ WLP (Θ := alloc.acc_alloc) (generate e G) (fun w1 θ '(t,ee) =>
                                    G[θ] |--ₚ e; t ~> ee).
   Proof.
-    induction e; cbn; intros w G; unfold T, _4; wsimpl.
-    - destruct lookup eqn:?; wsimpl.
-      constructor. intros ι _; pred_unfold.
+    induction e; cbn; intros w G; unfold T, _4; predsimpl.
+    - destruct lookup eqn:?; predsimpl. pred_unfold.
       constructor. now rewrite lookup_inst Heqo.
-    - constructor. intros ι _. pred_unfold. constructor.
-    - constructor. intros ι _. pred_unfold. constructor.
+    - pred_unfold. constructor.
+    - pred_unfold. constructor.
     - rewrite wlp_bind. unfold _4. cbn.
       iPoseProof (IHe1 w G) as "-#IH1". iRevert "IH1". clear IHe1.
       iApply (@wlp_mono alloc.acc_alloc). iIntros (w1 θ1 (t1 & e1')) "!> HT1".
@@ -201,33 +160,28 @@ Section Correctness.
       rewrite wlp_bind. unfold _4.
       iPoseProof (IHe3 w2 G[θ1 ⊙ θ2]) as "-#IH3". iRevert "IH3". clear IHe3.
       iApply (@wlp_mono alloc.acc_alloc). iIntros (w3 θ3 (t3 & e3')) "!> HT3". cbn.
-      iIntros "Heq1 Heq2". wsimpl.
-      iStopProof. constructor. intros ι (HT1 & HT2 & HT3 & Heq1 & Heq2).
-      pred_unfold. wsimpl. constructor; auto.
+      iIntros "Heq1 Heq2". predsimpl. iStopProof. pred_unfold.
+      intros (HT1 & HT2 & HT3 & Heq1 & Heq2). pred_unfold. constructor; auto.
 
-    - iIntros "!>".
-      rewrite wlp_bind. unfold _4. cbn - [step].
-      iPoseProof (IHe (w ▻ ctx.length w) (G[step] ,, x∷ṫy.var ctx.in_zero))
-                    as "-#IH". iRevert "IH". clear IHe.
+    - iIntros "!>". rewrite wlp_bind. unfold _4.
+      iPoseProof (IHe (w ▻ world.fresh w) (G[step] ,, x∷ṫy.var world.in_zero))
+        as "-#IH". iRevert "IH". clear IHe.
       iApply (@wlp_mono alloc.acc_alloc). iIntros (w1 θ1 (t1 & e1')).
-      iIntros "!> HT". rewrite persist_insert. wsimpl.
-      iStopProof. constructor. intros ι HT1. pred_unfold.
-      rewrite inst_insert in HT1. now constructor.
-    - rewrite wlp_bind. unfold _4. cbn.
+      iIntros "!> HT". predsimpl. iStopProof. pred_unfold. constructor.
+      pred_unfold. psimplnew.
+
+    - rewrite wlp_bind. unfold _4.
       iPoseProof (IHe _ (G ,, x∷lift t w)) as "-#IH". iRevert "IH". clear IHe.
-      iApply (@wlp_mono alloc.acc_alloc). iIntros (w1 θ1 (t1 & e1')) "!> HT". cbn.
-      rewrite persist_insert. wsimpl.
-      iStopProof. constructor. intros ι HT1. pred_unfold. wsimpl.
-      rewrite inst_insert inst_lift in HT1. now constructor.
+      iApply (@wlp_mono alloc.acc_alloc). iIntros (w1 θ1 (t1 & e1')) "!> HT".
+      predsimpl. iStopProof. pred_unfold. constructor. psimplnew.
     - rewrite wlp_bind. unfold _4.
       iPoseProof (IHe1 w G) as "-#IH". iRevert "IH". clear IHe1.
       iApply (@wlp_mono alloc.acc_alloc). iIntros (w1 r1 (t12 & e1')) "!> HT1".
       rewrite wlp_bind. unfold _4.
       iPoseProof (IHe2 w1 G[r1]) as "-#IH". iRevert "IH". clear IHe2.
-      iApply (@wlp_mono alloc.acc_alloc). iIntros (w2 r2 (t2 & e2')) "!> HT2 !>". cbn.
-      unfold _4. wsimpl.
-      iStopProof. constructor. intros ι (HT1 & HT2). pred_unfold. wsimpl.
-      econstructor; eauto.
+      iApply (@wlp_mono alloc.acc_alloc). iIntros (w2 r2 (t2 & e2')) "!> HT2 !>".
+      unfold _4. predsimpl. iStopProof. pred_unfold.
+      intros (HT1 & HT2). pred_unfold. econstructor; eauto.
   Qed.
 
   Lemma generate_sound (e : Exp) (w0 : World) (G0 : Ėnv w0) t0 e0 :
@@ -235,7 +189,7 @@ Section Correctness.
   Proof.
     iStartProof. rewrite wand_is_impl. rewrite wp_impl.
     iPoseProof (@generate_sound_aux e w0 G0) as "-#Hsound". iRevert "Hsound".
-    iApply (@wlp_mono alloc.acc_alloc). iIntros (w1 θ1 [t e']) "!> HT". wsimpl.
+    iApply (@wlp_mono alloc.acc_alloc). iIntros (w1 θ1 [t e']) "!> HT". predsimpl.
     iStopProof. constructor. intros ι HT Heq1 Heq2. now pred_unfold.
   Qed.
 
@@ -247,7 +201,7 @@ Section Correctness.
   Proof.
     induction T as [G x t Hres|G|G|G e1 e1' e2 e2' e3 e3' t _ IH1 _ IH2 _ IH3
       |G x t1 t2 e e' _ IH|G x t1 t2 e e' _ IH|G e1 t2 e1' e2 t1 e2' _ IH1 _ IH2];
-      intros w0 G0; wsimpl; unfold _4, Worlds.T.
+      intros w0 G0; predsimpl; unfold _4, Worlds.T.
 
     - constructor. intros ι. pred_unfold.
       intros _ ->.
@@ -256,60 +210,55 @@ Section Correctness.
       + injection Hres. cbn. intros <-. cbn. now pred_unfold.
       + discriminate Hres.
 
-    - iIntros "#HeqG".
-      rewrite wp_bind. unfold _4.
+    - iIntros "#HeqG". rewrite wp_bind. unfold _4.
       iPoseProof (IH1 w0 G0 with "HeqG") as "-#IH". clear IH1. iRevert "IH".
-      iApply (@wp_mono alloc.acc_alloc). iIntros (w1 r1 (t1 & e1'')) "!> (#Heq1 & #Heq2)". wsimpl.
-
-      rewrite wp_bind. unfold _4.
+      iApply (@wp_mono alloc.acc_alloc). iIntros (w1 r1 (t1 & e1'')) "!> (#Heq1 & #Heq2)".
+      predsimpl. rewrite wp_bind. unfold _4.
       iPoseProof (IH2 w1 G0[r1] with "HeqG") as "-#IH". clear IH2. iRevert "IH".
-      iApply (@wp_mono alloc.acc_alloc). iIntros (w2 r2 (t2 & e2'')) "!> (#Heq3 & #Heq4)". wsimpl.
-
-      rewrite wp_bind. unfold _4.
+      iApply (@wp_mono alloc.acc_alloc). iIntros (w2 r2 (t2 & e2'')) "!> (#Heq3 & #Heq4)".
+      predsimpl. rewrite wp_bind. unfold _4.
       iPoseProof (IH3 w2 G0 with "HeqG") as "-#IH". clear IH3. iRevert "IH".
-      iApply (@wp_mono alloc.acc_alloc). iIntros (w3 r3 (t3 & e3'')) "!> (#Heq5 & #Heq6)". wsimpl.
-
+      iApply (@wp_mono alloc.acc_alloc). iIntros (w3 r3 (t3 & e3'')) "!> (#Heq5 & #Heq6)".
+      predsimpl.
       iStopProof. constructor. intros ι [_ [(HeqG & Heq1 & Heq2 & Heq3 & Heq4 & Heq5 & Heq6)]].
-      pred_unfold. wsimpl. now subst.
+      pred_unfold. psimplnew.
 
     - iIntros "#HeqG". rewrite Acc.intro_wp_step. iExists (lift t1 _). iIntros "!> #Heq1".
-      rewrite wp_bind. unfold _4. wsimpl.
-      iPoseProof (IH _ (G0 ,, x∷ṫy.var ctx.in_zero)) as "IH". clear IH. wsimpl.
-      rewrite <- eqₚ_insert. wsimpl.
+      rewrite wp_bind. unfold _4. predsimpl.
+      iPoseProof (IH _ (G0 ,, x∷ṫy.var world.in_zero)) as "IH". clear IH. predsimpl.
       iPoseProof ("IH" with "HeqG Heq1") as "-#IH'"; iClear "IH". iRevert "IH'".
       iApply (@wp_mono alloc.acc_alloc).
-      iIntros (w1 r1 (t2' & e1'')) "!> (#Heq2 & #Heq3)"; wsimpl.
+      iIntros (w1 r1 (t2' & e1'')) "!> (#Heq2 & #Heq3)"; predsimpl.
       repeat iSplit; auto.
       iStopProof. constructor. intros ι [_ [(HeqG & Heq1 & Heq2 & Heq3)]].
-      pred_unfold. wsimpl. now subst.
+      pred_unfold. psimplnew.
 
     - iIntros "#HeqG".
       rewrite wp_bind. unfold _4.
-      iPoseProof (IH _ (G0 ,, x∷lift t1 w0)) as "IH". clear IH. wsimpl.
-      rewrite <- eqₚ_insert. wsimpl.
+      iPoseProof (IH _ (G0 ,, x∷lift t1 w0)) as "IH". clear IH. predsimpl.
       iPoseProof ("IH" with "HeqG") as "-#IH'"; iClear "IH". iRevert "IH'".
       iApply (@wp_mono alloc.acc_alloc).
-      iIntros (w1 r1 (t2' & e'')) "!> (#Heq1 & #Heq2)"; wsimpl.
+      iIntros (w1 r1 (t2' & e'')) "!> (#Heq1 & #Heq2)"; predsimpl.
       iSplit; auto.
       iStopProof. constructor. intros ι [_ [(HeqG & Heq1 & Heq2)]].
-      pred_unfold. wsimpl. now subst.
+      pred_unfold. psimplnew.
 
     - iIntros "#HeqG".
-      rewrite wp_bind. unfold _4. wsimpl.
-      iPoseProof (IH1 _ G0) as "IH"; clear IH1. wsimpl.
+      rewrite wp_bind. unfold _4. predsimpl.
+      iPoseProof (IH1 _ G0) as "IH"; clear IH1. predsimpl.
       iPoseProof ("IH" with "HeqG") as "-#IH'"; iClear "IH". iRevert "IH'".
       iApply (@wp_mono alloc.acc_alloc).
-      iIntros (w1 r1 (tf & e1'')) "!> (#Heq1 & #Heq2)"; wsimpl.
+      iIntros (w1 r1 (tf & e1'')) "!> (#Heq1 & #Heq2)"; predsimpl.
 
       rewrite wp_bind. unfold _4.
       iPoseProof (IH2 w1 G0 with "HeqG") as "-#IH"; clear IH2. iRevert "IH".
       iApply (@wp_mono alloc.acc_alloc).
-      iIntros (w2 r2 (t1' & e2'')) "!> (#Heq3 & #Heq4)"; wsimpl.
-      rewrite Acc.intro_wp_step. iExists (lift t2 w2). unfold _4. rewrite lk_refl. wsimpl.
-      iIntros "!>". wsimpl.
+      iIntros (w2 r2 (t1' & e2'')) "!> (#Heq3 & #Heq4)"; predsimpl.
+      rewrite Acc.intro_wp_step. iExists (lift t2 w2). unfold _4. predsimpl.
+      iIntros "!>". predsimpl.
 
       iStopProof. constructor. intros ι [_ [(HeqG & Heq1 & Heq2 & Heq3 & Heq4)]].
-      pred_unfold. wsimpl. now subst.
+      pred_unfold. psimplnew.
   Qed.
 
   Lemma generate_complete (e : Exp) (w0 : World) (G0 : Ėnv w0) t0 e0 :
@@ -319,8 +268,8 @@ Section Correctness.
     destruct (@generate_complete_aux _ _ _ _ HT w0 G0) as [Hcompl].
     specialize (Hcompl ι (MkEmp _)). pred_unfold.
     specialize (Hcompl eq_refl). revert Hcompl.
-    apply wp_mono. intros w1 θ1 [t1 e1].
-    wsimpl. intros ι1 <-. pred_unfold. wsimpl.
+    apply wp_mono. intros w1 θ1 [t1 e1]. cbn.
+    intros ι1 <-. pred_unfold. psimplnew.
   Qed.
 
   Lemma generate_correct (e : Exp) (w0 : World) (G0 : Ėnv w0) t0 e0 :
@@ -330,7 +279,7 @@ Section Correctness.
   Import (hints) Triangular.Tri.
   Import (hints) Acc.
 
-  Definition TPB_OD (e : Exp) (t : Ty) (ee : Exp) : Pred ctx.nil :=
+  Definition TPB_OD (e : Exp) (t : Ty) (ee : Exp) : Pred world.nil :=
     wp_optiondiamond (reconstruct_optiondiamond e)
       (fun w θ '(t', ee') => t' =ₚ lift t w /\ₚ ee' =ₚ lift ee w).
 
@@ -356,7 +305,7 @@ Section Correctness.
     rewrite <- solver_correct.
     unfold wp_optiondiamond.
     destruct (solver C) as [(w2 & θ2 & [])|]; cbn.
-    - rewrite Acc.and_wp_l. wsimpl. clear.
+    - rewrite Acc.and_wp_l. predsimpl.
       rewrite eqₚ_sym.
       generalize (t' =ₚ lift t w2). clear. intros P.
       rewrite eqₚ_sym.
@@ -369,8 +318,8 @@ Section Correctness.
   Qed.
 
   Definition tpb_algo (e : Exp) (t : Ty) (ee : Exp) : Prop :=
-    match reconstruct_schematic e with
-    | Some (existT w (t', ee')) =>
+    match reconstruct_optiondiamond e with
+    | Some (existT w (_ , (t', ee'))) =>
         exists ι : Assignment w, inst t' ι = t /\ inst ee' ι = ee
     | None => False
     end.
@@ -379,7 +328,7 @@ Section Correctness.
     tpb empty e t ee <-> tpb_algo e t ee.
   Proof.
     generalize (reconstruct_schematic_correct e t ee).
-    unfold TPB_OD, tpb_algo, reconstruct_schematic.
+    unfold TPB_OD, tpb_algo.
     intros [HE]. specialize (HE env.nil). pred_unfold.
     rewrite inst_empty in HE. rewrite HE. clear HE.
     destruct reconstruct_optiondiamond as [(w & θ & [t' ee'])|]; cbn; auto.
