theories/Stlc/Unification.v
@@ -41,7 +41,7 @@ From Em Require Import
   Stlc.Triangular
   Stlc.Worlds.
 
-Import Pred ctx.notations Tri.notations World.notations Pred.notations.
+Import Pred world.notations World.notations Pred.notations.
 Import (hints) Diamond Sub Tri.
 
 Set Implicit Arguments.
@@ -53,28 +53,87 @@ Notation OptionDiamond := (DiamondT Tri Option).
     (at level 8, left associativity,
       format "s [ ζ ]").
 
-Ltac folddefs :=
-  repeat
-    match goal with
-    | |- context[@Tri.refl ?w] =>
-        change_no_check (@Tri.refl w) with (@refl Tri _ w)
-    | |- context[Tri.cons ?x ?t refl] =>
-        change_no_check (Tri.cons x t refl) with (thick x t)
-    | |- context[Tri.cons ?x ?t ?r] =>
-        change_no_check (Tri.cons x t r) with (thick x t ⊙⁻ r)
+#[local] Notation "▷ A" :=
+  (fun (w : World) => forall α (αIn : α ∈ w), A (w - α))
+    (at level 9, right associativity).
+#[local] Notation "▶ P" :=
+  (fun w (d : ▷_ w) => forall α (αIn : α ∈ w), P (w - α) (d α αIn))
+    (at level 9, right associativity).
+
+(* In this section we define a generic Bove-Capretta style accessibility
+   predicate for functions that recurse on smaller contexts by removing an
+   element.
+
+   See: BOVE, ANA, and VENANZIO CAPRETTA. “Modelling General Recursion in
+   Type Theory.” Mathematical Structures in Computer Science, vol. 15,
+   no. 4, 2005, pp. 671–708., doi:10.1017/S0960129505004822. *)
+Section RemoveAcc.
+
+  (* Coq only generates non-dependent elimination schemes for inductive
+     families in Prop. Hence, we disable the automatic generation and
+     define the elimination schemes for the predicate ourselves. *)
+  #[local] Unset Elimination Schemes.
+
+  Inductive remove_acc (w : World) : Prop :=
+    remove_acc_intro : ▷remove_acc w -> remove_acc w.
+
+  Definition remove_acc_inv {w} (d : remove_acc w) : ▷remove_acc w :=
+    let (f) := d in f.
+
+  (* We only define a non-dependent elimination scheme for Type. *)
+  Definition remove_acc_rect (P : forall Γ, Type)
+    (f : forall w, ▷P w -> P w) :
+    forall w, remove_acc w -> P w :=
+    fix F w (d : remove_acc w) {struct d} : P w :=
+      f w (fun α αIn => F (w - α) (remove_acc_inv d αIn)).
+
+  (* Define a dependent elimination scheme for Prop. *)
+  Definition remove_acc_ind (P : forall w, remove_acc w -> Prop)
+    (f : forall w (d : ▷remove_acc w), ▶P w d -> P w (remove_acc_intro d)) :=
+    fix F w (d : remove_acc w) {struct d} : P w d :=
+      let (g) return _ := d in
+      f w g (fun x xIn => F (w - x) (g x xIn)).
+
+  Fixpoint remove_acc_step {w α} (r : remove_acc w) {struct r} :
+    remove_acc (world.snoc w α) :=
+    remove_acc_intro
+      (fun β (βIn : β ∈ (world.snoc w α)) =>
+         match world.view βIn in @world.SnocView _ _ β βIn
+               return remove_acc (world.snoc w α - β) with
+         | world.isZero   => r
+         | world.isSucc i => remove_acc_step (remove_acc_inv r i)
+         end).
+
+  Fixpoint remove_acc_all (w : World) : remove_acc w :=
+    match w with
+    | world.nil      => remove_acc_intro
+                        (fun x (xIn : x ∈ world.nil) =>
+                           match world.view xIn with end)
+    | world.snoc w b => remove_acc_step (remove_acc_all w)
     end.
 
-Definition löb {A} : (⊢ʷ ▷A -> A) -> (⊢ʷ A) :=
-  fun step w => ctx.remove_acc_rect A step (ctx.remove_acc_all w).
+  (* Calculating the full predicate is costly. It has quadratic running
+     time in the size of the context. It's better to keep this opaque and
+     not unfold it. To prevent computation from being blocked, clients of
+     this code should never pattern match on a witness of the predicate
+     directly and instead use [remove_acc_inv] in the recursive call. The
+     standard library uses the same style and for examples defines [Fix_F]
+     for well-founded induction using [Acc_inv] for recursive calls. *)
+  #[global] Opaque remove_acc_all.
 
-Definition löb_elim {A} (step : ⊢ʷ ▷A -> A) (P : forall w, A w -> Prop)
-  (IH: forall w (f : ▷A w) (pf : forall x xIn, P (w - x) (f x xIn)), P w (step w f)) :
-  forall w, P w (löb step w).
-Proof. intros w. unfold löb. induction (ctx.remove_acc_all w). now apply IH. Qed.
+  Definition löb {A : World -> Type} : (⊧ ▷A ̂→ A)%W -> (⊧ A) :=
+    fun step w => remove_acc_rect A step (remove_acc_all w).
+
+  Definition löb_elim {A} (step : ⊧ ▷A ̂→ A) (P : forall w, A w -> Prop)
+    (IH: forall w (f : ▷A w) (pf : forall x xIn, P (w - x) (f x xIn)), P w (step w f)) :
+    forall w, P w (löb step w).
+  Proof. intros w. unfold löb. induction (remove_acc_all w). now apply IH. Qed.
+
+End RemoveAcc.
 
 Section Operations.
 
-  Definition fail {A} : ⊢ʷ OptionDiamond A :=
+  Definition fail {A} : ⊧ OptionDiamond A :=
     fun w => None.
   #[global] Arguments fail {A w}.
 
@@ -88,14 +147,14 @@ Section OccursCheck.
   Import option.notations.
   Import (hints) Sub.
 
-  Definition occurs_check_in : ⊢ʷ ∀ x, ctx.In x -> ▷(Option (ctx.In x)) :=
+  Definition occurs_check_in : ⊧ ∀ x, world.In x ̂→ ▷(Option (world.In x)) :=
     fun w x xIn y yIn =>
-      match ctx.occurs_check_view yIn xIn with
-      | ctx.Same _      => None
-      | ctx.Diff _ xIn' => Some xIn'
+      match world.occurs_check_view yIn xIn with
+      | world.Same _      => None
+      | world.Diff _ xIn' => Some xIn'
       end.
 
-  Definition occurs_check : ⊢ʷ Ṫy -> ▷(Option Ṫy) :=
+  Definition occurs_check : ⊧ Ṫy ̂→ ▷(Option Ṫy) :=
     fun w =>
       fix oc (t : Ṫy w) β (βIn : β ∈ w) {struct t} :=
       match t with
@@ -105,22 +164,22 @@ Section OccursCheck.
       end.
 
   Lemma occurs_check_spec {w α} (αIn : α ∈ w) (t : Ṫy w) :
-    option.spec
-      (fun t' => t = t'[thin α])
-      (t = ṫy.var αIn \/ ṫy.Ṫy_subterm (ṫy.var αIn) t)
-      (occurs_check t αIn).
+    match occurs_check t αIn with
+    | Some t' => t = t'[thin α]
+    | None => t = ṫy.var αIn \/ ṫy.Ṫy_subterm (ṫy.var αIn) t
+    end.
   Proof.
     induction t; cbn.
     - unfold occurs_check_in.
-      destruct (ctx.occurs_check_view αIn αIn0); constructor.
+      destruct (world.occurs_check_view αIn αIn0); cbn.
       + left. reflexivity.
-      + cbn. now rewrite lk_thin.
-    - constructor. reflexivity.
-    - repeat option.tactics.mixin; subst; auto; right;
+      + now rewrite lk_thin.
+    - reflexivity.
+    - destruct (occurs_check t1 αIn), (occurs_check t2 αIn); cbn; subst; auto; right;
         match goal with
-        | H: _ \/ ṫy.Ṫy_subterm _ ?t |- _ =>
-            destruct H;
-            [ subst; constructor; constructor
+               | H: _ \/ ṫy.Ṫy_subterm _ ?t |- _ =>
+                   destruct H;
+                   [ subst; constructor; constructor
             | constructor 2 with t; auto; constructor; constructor
             ]
         end.
@@ -147,26 +206,26 @@ Section Implementation.
 
   Definition C := Box Tri (OptionDiamond Unit).
 
-  Definition ctrue : ⊢ʷ C :=
+  Definition ctrue : ⊧ C :=
     fun w0 w1 r01 => pure tt.
-  Definition cfalse : ⊢ʷ C :=
+  Definition cfalse : ⊧ C :=
     fun w0 w1 r01 => fail.
-  Definition cand : ⊢ʷ C -> C -> C :=
+  Definition cand : ⊧ C ̂→ C ̂→ C :=
     fun w0 c1 c2 w1 r01 =>
       bind (c1 w1 r01) (fun w2 r12 _ => _4 c2 r01 r12).
   #[global] Arguments cfalse {w} [w1] _.
   #[global] Arguments ctrue {w} [w1] _.
 
   Definition BoxUnifier : TYPE :=
-    Ṫy -> Ṫy -> C.
+    Ṫy ̂→ Ṫy ̂→ C.
 
-  Definition flex : ⊢ʷ ∀ α, ctx.In α -> Ṫy -> OptionDiamond Unit :=
+  Definition flex : ⊧ ∀ α, world.In α ̂→ Ṫy ̂→ OptionDiamond Unit :=
     fun w α αIn τ =>
       match varview τ with
       | is_var βIn =>
-          match ctx.occurs_check_view αIn βIn with
-          | ctx.Same _      => pure tt
-          | ctx.Diff _ βIn' => singleton αIn (ṫy.var βIn')
+          match world.occurs_check_view αIn βIn with
+          | world.Same _      => pure tt
+          | world.Diff _ βIn' => singleton αIn (ṫy.var βIn')
           end
       | not_var _ =>
           match occurs_check τ αIn with
@@ -184,12 +243,12 @@ Section Implementation.
     Definition aflex α {αIn : α ∈ w} (τ : Ṫy w) : C w :=
       fun _ θ =>
         match θ with
-        | Tri.refl         => flex α τ
+        | Tri.nil          => flex α τ
         | Tri.cons β τ' θ' => lamgu (lk (thick β τ') αIn) τ[thick β τ'] θ'
         end.
     #[global] Arguments aflex α {αIn} τ [w1] _.
 
-    Definition atrav : (Ṫy -> Ṫy -> C)%W w :=
+    Definition atrav : (Ṫy ̂→ Ṫy ̂→ C)%W w :=
       fix bmgu s t {struct s} :=
         match s , t with
         | @ṫy.var _ α _  , t             => aflex α t
@@ -220,36 +279,29 @@ Section Implementation.
 
   End MguO.
 
-  Definition amgu : ⊢ʷ BoxUnifier :=
+  Definition amgu : ⊧ BoxUnifier :=
     löb atrav.
 
-  Definition mgu : ⊢ʷ Ṫy -> Ṫy -> OptionDiamond Unit :=
+  Definition mgu : ⊧ Ṫy ̂→ Ṫy ̂→ OptionDiamond Unit :=
     fun w s t => T (@amgu w s t).
 
-  Definition asolver : ⊢ʷ List (Prod Ṫy Ṫy) -> C :=
+  Definition asolver : ⊧ List (Prod Ṫy Ṫy) ̂→ C :=
     fix asolver {w} cs {struct cs} :=
       match cs with
       | List.nil             => ctrue
       | List.cons (t1,t2) cs => cand (amgu t1 t2) (asolver cs)
       end.
 
-  Definition solver : ⊢ʷ List (Prod Ṫy Ṫy) -> OptionDiamond Unit :=
+  Definition solver : ⊧ List (Prod Ṫy Ṫy) ̂→ OptionDiamond Unit :=
     fun w cs => asolver cs refl.
 
-  Import option.notations.
-
   Definition solveoptiondiamond {A} {pA : Persistent A} :
-    Diamond alloc.acc_alloc (List (Ṫy * Ṫy) * A) ctx.nil ->
-    Option (Diamond alloc.acc_alloc A) ctx.nil :=
+    Diamond alloc.acc_alloc (List (Ṫy * Ṫy) * A) world.nil ->
+    Option (Diamond alloc.acc_alloc A) world.nil :=
     fun '(existT w1 (θ1, (cs, a))) =>
-      '(existT w2 (θ2, tt))      <- solver cs;;
-      Some (existT w2 (alloc.nil_l,persist a θ2)).
-
-  Definition optiondiamond2schematic {A} :
-    Option (Diamond alloc.acc_alloc A) ctx.nil ->
-    option (Schematic A) :=
-      option.map
-        (fun '(existT w (θ,a)) => existT w a).
+      option.bind (solver cs)
+        (fun '(existT w2 (θ2, tt)) =>
+           Some (existT w2 (alloc.nil,persist a θ2))).
 
 End Implementation.
 
@@ -274,7 +326,7 @@ Section Correctness.
     cbn. rewrite and_true_l, <- persist_pred_trans. apply H2.
   Qed.
 
-  Definition BoxUnifierCorrect : ⊢ʷ BoxUnifier -> PROP :=
+  Definition BoxUnifierCorrect : ⊧ BoxUnifier ̂→ PROP :=
     fun w0 bu =>
       forall (t1 t2 : Ṫy w0) w1 (θ1 : w0 ⊒⁻ w1),
         instpred (bu t1 t2 w1 θ1) ⊣⊢ₚ (t1 =ₚ t2)[θ1].
@@ -283,14 +335,15 @@ Section Correctness.
     instpred (flex α t) ⊣⊢ₚ ṫy.var αIn =ₚ t.
   Proof.
     unfold flex. destruct varview; cbn.
-    - destruct ctx.occurs_check_view; cbn.
+    - destruct world.occurs_check_view; cbn.
       + now rewrite Acc.wp_refl, eqₚ_refl.
       + rewrite Acc.wp_thick, persist_true, and_true_r.
         cbn. now rewrite lk_thin.
-    - destruct (occurs_check_spec αIn t) as [|[HOC|HOC]]; cbn.
+    - pose proof (occurs_check_spec αIn t) as HOC. destruct occurs_check; cbn.
       + subst. now rewrite Acc.wp_thick, persist_true, and_true_r.
-      + subst. now contradiction (H α αIn).
-      + apply pno_cycle in HOC. apply split_bientails. now split.
+      + destruct HOC as [HOC|HOC].
+        * subst. now contradiction (H α αIn).
+        * apply pno_cycle in HOC. apply split_bientails. now split.
   Qed.
 
   Section InnerRecursion.
@@ -302,7 +355,8 @@ Section Correctness.
     Lemma aflex_correct {α} (αIn : α ∈ w) (t : Ṫy w) w1 (θ1 : w ⊒⁻ w1) :
       instpred (aflex lamgu α t θ1) ⊣⊢ₚ (ṫy.var αIn =ₚ t)[θ1].
     Proof.
-      destruct θ1; cbn; folddefs.
+      destruct θ1; cbn; Tri.folddefs.
+      Tri.folddefs.
       - now rewrite flex_correct, persist_pred_refl.
       - now rewrite lamgu_correct, !persist_eq, !persist_trans.
     Qed.
