theories/common/Environment.v
@@ -26,658 +26,146 @@
 (* SOFTWARE, EVEN IF ADVISED OF THE POSSIBILITY OF SUCH DAMAGE.               *)
 (******************************************************************************)
 
-From Coq Require Import
-     Bool.Bool.
-From Equations Require Import Equations.
-
 From Em Require Import
      Context Prelude.
-Import ctx.notations.
+Import world.notations.
 
-Local Set Implicit Arguments.
-Local Open Scope lazy_bool_scope.
-Local Unset Equations Derive Equations.
+#[local] Set Implicit Arguments.
 
 Declare Scope env_scope.
 Delimit Scope env_scope with env.
-Declare Scope dep_pattern_scope.
-Delimit Scope dep_pattern_scope with dep_pattern.
 
 Module env.
 
 Section WithBinding.
-  Context {B : Set}.
 
   Section WithDom.
-    Context {D : B -> Set}.
+    Context {D : Set}.
 
-    Inductive Env : Ctx B -> Set :=
-    | nil                                     : Env []
-    | snoc {Γ} (E : Env Γ) {b : B} (db : D b) : Env (Γ ▻ b).
+    Inductive Env : World → Set :=
+    | nil                              : Env []
+    | snoc {w} (E : Env w) {α} (d : D) : Env (w ▻ α).
 
-    Variant NilView : Env [] -> Set :=
+    Variant NilView : Env [] → Set :=
       isNil : NilView nil.
 
-    Variant SnocView {Γ b} : Env (Γ ▻ b) -> Set :=
-      isSnoc (E : Env Γ) (v : D b) : SnocView (snoc E v).
+    Variant SnocView {w α} : Env (w ▻ α) → Set :=
+      isSnoc (E : Env w) (v : D) : SnocView (snoc E v).
 
-    Definition view (Γ : Ctx B) (E : Env Γ) :
-      match Γ with
-      | [ctx] => NilView
-      | Γ ▻ b => SnocView
+    Definition view (w : World) (E : Env w) :
+      match w with
+      | []    => NilView
+      | w ▻ α => SnocView
       end E :=
       match E with
       | nil      => isNil
       | snoc E v => isSnoc E v
       end.
 
-    Fixpoint cat {Γ Δ} (EΓ : Env Γ) (EΔ : Env Δ) : Env (Γ ▻▻ Δ) :=
-      match EΔ with
-      | nil       => EΓ
-      | snoc E db => snoc (cat EΓ E) db
-      end.
-
-    Variant CatView {Γ Δ} : Env (Γ ▻▻ Δ) -> Set :=
-      isCat (EΓ : Env Γ) (EΔ : Env Δ) : CatView (cat EΓ EΔ).
-
-    Fixpoint catView {Γ Δ} : forall E : Env (Γ ▻▻ Δ), CatView E :=
-      match Δ as c return forall E : Env (Γ ▻▻ c), CatView E with
-      | [ctx] => fun EΓ : Env Γ => isCat EΓ nil
-      | Δ ▻ b => fun EΓΔb : Env (Γ ▻▻ Δ ▻ b) =>
-                   let '(isSnoc EΓΔ v) := view EΓΔb in
-                   let '(isCat EΓ EΔ)  := catView EΓΔ in
-                   isCat EΓ (snoc EΔ v)
-      end.
-
-    Lemma catView_cat {Γ Δ} (EΓ : Env Γ) (EΔ : Env Δ) :
-      catView (cat EΓ EΔ) = isCat EΓ EΔ.
-    Proof. induction EΔ; cbn; now rewrite ?IHEΔ. Qed.
-
-    Ltac destroy x :=
-      try (progress cbn in x);
-      lazymatch type of x with
-      | Env []       => destruct (view x)
-      | Env (_ ▻ _)  => destruct (view x) as [x]; destroy x
-      | Env (_ ▻▻ _) => let E1 := fresh in
-                        let E2 := fresh in
-                        destruct (catView x) as [E1 E2];
-                        destroy E1; destroy E2
-      | _ ∈ []       => destruct (ctx.view x)
-      | _ ∈ _ ▻ _    => destruct (ctx.view x)
-      | _            => idtac
-      end.
-
-    Section TransparentObligations.
-      Local Set Transparent Obligations.
-      Derive Signature NoConfusion NoConfusionHom for Env.
-
-      Context {eqdec_b : EqDec B}.
-      Context {eqdec_d : forall b, EqDec (D b) }.
-
-      #[export] Instance eq_dec_env {Γ} : EqDec (Env Γ).
-      Proof. eqdec_proof. Defined.
-
-    End TransparentObligations.
-
-    Section Inversions.
-
-      Lemma inversion_eq_snoc {Γ : Ctx B} {b : B} (E1 E2 : Env Γ) (v1 v2 : D b) :
-        snoc E1 v1 = snoc E2 v2 <->
-        E1 = E2 /\ v1 = v2.
-      Proof.
-        split.
-        - intros H. now dependent elimination H.
-        - intros []; congruence.
-      Qed.
-
-      Lemma inversion_eq_cat {Γ Δ : Ctx B} (EΓ1 EΓ2 : Env Γ) (EΔ1 EΔ2 : Env Δ) :
-        cat EΓ1 EΔ1 = cat EΓ2 EΔ2 <->
-        EΓ1 = EΓ2 /\ EΔ1 = EΔ2.
-      Proof.
-        induction EΔ1; destroy EΔ2; cbn; [easy|].
-        now rewrite !inversion_eq_snoc, IHEΔ1.
-      Qed.
-
-    End Inversions.
-
-    Fixpoint lookup {Γ} (E : Env Γ) : forall {b}, b ∈ Γ -> D b :=
+    Fixpoint lookup {w} (E : Env w) : ∀ [α], α ∈ w → D :=
       match E with
-      | nil      => fun _ bIn => match ctx.view bIn with end
-      | snoc E v => fun _ bIn =>
-        match ctx.view bIn with
-        | ctx.isZero   => v
-        | ctx.isSucc i => lookup E i
-        end
+      | nil      => fun _ αIn => match world.view αIn with end
+      | snoc E v => fun _ αIn => match world.view αIn with
+                                 | world.isZero      => v
+                                 | world.isSucc αIn' => lookup E αIn'
+                                 end
       end.
 
-    Inductive All (Q : forall b, D b -> Type) : forall {Γ}, Env Γ -> Type :=
-    | all_nil : All Q nil
-    | all_snoc {Γ E b d} : @All Q Γ E -> Q b d -> All Q (snoc E d).
-
-    #[derive(equations=no)]
-    Equations all_snoc_inv_1 {Q : forall b, D b -> Type} {Γ b} {E : Env Γ} {d : D b} :
-      All Q (snoc E d) -> All Q E := | all_snoc QE _ => QE.
-
-    #[derive(equations=no)]
-    Equations all_snoc_inv_2 {Q : forall b, D b -> Type} {Γ b} {E : Env Γ} {d : D b} :
-      All Q (snoc E d) -> Q b d := | all_snoc _ Qd => Qd.
-
-    Lemma all_intro {Q : forall [b], D b -> Type} (HQ : forall b (d : D b), Q d) :
-      forall Γ (E : Env Γ), All Q E.
-    Proof. intros ? E. induction E; constructor; auto. Defined.
-
-    Lemma all_elim {Q : forall [b], D b -> Type} {Γ} {E : Env Γ} (HE : All Q E) :
-      forall b (bIn : b ∈ Γ), Q (lookup E bIn).
-    Proof. induction HE; intros x xIn; destruct (ctx.view xIn); cbn; auto. Defined.
-
-    Section HomEquality.
-
-      Variable eqb : forall [b], D b -> D b -> bool.
-
-      Equations(noeqns) eqb_hom {Γ} (δ1 δ2 : Env Γ) : bool :=
-      | nil         | nil         := true;
-      | snoc δ1 db1 | snoc δ2 db2 := eqb db1 db2 &&& eqb_hom δ1 δ2.
-
-      (* Lemma eqb_hom_spec_point (Γ : Ctx B) (xs : Env Γ) *)
-      (*   (HYP : All (fun b => EqbSpecPoint (@eqb b)) xs) : *)
-      (*   EqbSpecPoint eqb_hom xs. *)
-      (* Proof. *)
-      (*   induction xs; intros ys; destroy ys; cbn. *)
-      (*   - do 2 constructor. *)
-      (*   - specialize (IHxs (all_snoc_inv_1 HYP)). pose proof (all_snoc_inv_2 HYP) as IHb. *)
-      (*     destruct (IHb v); subst. *)
-      (*     + destruct IHxs with ys; constructor. *)
-      (*       * subst; auto. *)
-      (*       * intros ?%inversion_eq_snoc. intuition. *)
-      (*     + constructor. intros ?%inversion_eq_snoc. intuition. *)
-      (* Qed. *)
-
-      (* Variable eqb_spec : forall b (x y : D b), *)
-      (*   reflect (x = y) (eqb x y). *)
-
-      (* Lemma eqb_hom_spec {Γ} (δ1 δ2 : Env Γ) : *)
-      (*   reflect (δ1 = δ2) (eqb_hom δ1 δ2). *)
-      (* Proof. apply eqb_hom_spec_point, all_intro; auto. Qed. *)
-
-    End HomEquality.
-
-    Section HetEquality.
-
-      Variable eqb : forall b1 b2, D b1 -> D b2 -> bool.
-
-      Fixpoint eqb_het {Γ1 Γ2} (δ1 : Env Γ1) (δ2 : Env Γ2) {struct δ1} : bool :=
-        match δ1 , δ2 with
-        | nil         , nil         => true
-        | snoc δ1 db1 , snoc δ2 db2 => eqb db1 db2 &&& eqb_het δ1 δ2
-        | _           , _           => false
-        end.
-
-      (* Variable eqb_spec : forall b1 b2 (x : D b1) (y : D b2), *)
-      (*     reflect ({| pr2 := x |} = {| pr2 := y |}) (eqb x y). *)
-
-      (* Lemma eqb_het_spec {Γ1 Γ2} (δ1 : Env Γ1) (δ2 : Env Γ2) : *)
-      (*   reflect ({| pr2 := δ1 |} = {| pr2 := δ2 |}) (eqb_het δ1 δ2). *)
-      (* Proof. *)
-      (*   revert Γ2 δ2; induction δ1; intros ? []; cbn. *)
-      (*   - constructor. reflexivity. *)
-      (*   - constructor. intro e; dependent elimination e. *)
-      (*   - constructor. intro e; dependent elimination e. *)
-      (*   - destruct (eqb_spec db db0). *)
-      (*     + apply (ssrbool.iffP (IHδ1 _ E)); intros Heq; dependent elimination Heq. *)
-      (*       * dependent elimination e; reflexivity. *)
-      (*       * reflexivity. *)
-      (*     + constructor; intros e; dependent elimination e; congruence. *)
-      (* Qed. *)
-
-    End HetEquality.
-
-    (* ! *)
-    Fixpoint tabulate {Γ} : (forall b, b ∈ Γ -> D b) -> Env Γ :=
-      match Γ with
+    Fixpoint tabulate {w} : (∀ α, α ∈ w → D) → Env w :=
+      match w with
       | []    => fun _ => nil
-      | Γ ▻ b => fun EΓb =>
-        snoc (tabulate (fun y yIn => EΓb y (ctx.in_succ yIn))) (EΓb _ ctx.in_zero)
+      | w ▻ α => fun Ewα =>
+                   snoc
+                     (tabulate (fun β βIn => Ewα β (world.in_succ βIn)))
+                     (Ewα _ world.in_zero)
       end.
 
-    Fixpoint update {Γ} (E : Env Γ) {struct E} :
-      forall {b} (bIn : b ∈ Γ) (new : D b), Env Γ :=
+    Fixpoint remove {Γ b} (E : Env Γ) : ∀ (bIn : b ∈ Γ), Env (Γ - b) :=
       match E with
-      | nil        => fun _ bIn => match ctx.view bIn with end
-      | snoc E old => fun _ bIn =>
-        match ctx.view bIn with
-        | ctx.isZero     => snoc E
-        | ctx.isSucc bIn => fun new => snoc (update E bIn new) old
-        end
-      end.
-
-    Definition head {Γ b} (E : Env (Γ ▻ b)) : D b :=
-      match E in Env Γb
-      return match Γb with
-             | []    => unit
-             | Γ ▻ b => D b
-             end
-      with
-      | nil => tt
-      | snoc E db => db
-      end.
-
-    Definition tail {Γ b} (E : Env (Γ ▻ b)) : Env Γ :=
-      match E in Env Γb
-      return match Γb with
-             | []    => unit
-             | Γ ▻ _ => Env Γ
-             end
-      with
-      | nil => tt
-      | snoc E _ => E
-      end.
-
-    Fixpoint take {Γ} Δ (E : Env (Γ ▻▻ Δ)) : Env Δ :=
-      match Δ , E with
-      | []    , E => nil
-      | Δ ▻ b , E => snoc (take Δ (tail E)) (head E)
-      end.
-
-    Fixpoint drop {Γ} Δ (E : Env (Γ ▻▻ Δ)) : Env Γ :=
-      match Δ , E with
-      | []    , E => E
-      | Δ ▻ _ , E => drop Δ (tail E)
-      end.
-
-    Fixpoint remove {Γ b} (E : Env Γ) : forall (bIn : b ∈ Γ), Env (Γ - b) :=
-      match E with
-      | nil      => fun bIn => match ctx.view bIn with end
+      | nil      => fun bIn => match world.view bIn with end
       | snoc E d => fun bIn =>
-                      match ctx.view bIn return Env (_ - _) with
-                      | ctx.isZero => E
-                      | ctx.isSucc i => snoc (remove E i) d
+                      match world.view bIn return Env (_ - _) with
+                      | world.isZero => E
+                      | world.isSucc i => snoc (remove E i) d
                       end
       end.
-    Global Arguments remove {_} b%ctx E.
+    #[global] Arguments remove {_} b E.
 
-    Fixpoint insert {Γ b} (bIn : b ∈ Γ) : Env (Γ - b) -> D b -> Env Γ :=
+    Fixpoint insert {Γ b} (bIn : b ∈ Γ) : Env (Γ - b) → D → Env Γ :=
       match bIn with
-      | ctx.in_zero     => fun E v => snoc E v
-      | ctx.in_succ bIn => fun E v =>
-        match view E with
-        | isSnoc E v' => snoc (insert bIn E v) v'
-        end
+      | world.in_zero     => fun E v => snoc E v
+      | world.in_succ bIn => fun E v =>
+        let (E,v') := view E in
+        snoc (insert bIn E v) v'
       end.
 
-    Lemma remove_insert {b} {Γ} (bIn : b ∈ Γ) (v : D b) (E : Env (Γ - b)) :
+    Lemma remove_insert {b} {Γ} (bIn : b ∈ Γ) (v : D) (E : Env (Γ - b)) :
       remove b (insert bIn E v) bIn = E.
-    Proof. induction Γ; destroy bIn; destroy E; cbn; now f_equal. Qed.
+    Proof. induction bIn; cbn in *. easy. destruct view. cbn. now f_equal. Qed.
 
     Lemma insert_remove {b} {Γ} (bIn : b ∈ Γ) (E : Env Γ) :
       insert bIn (remove b E bIn) (lookup E bIn) = E.
-    Proof. induction E; destroy bIn; cbn; now f_equal. Qed.
+    Proof. induction E; destruct (world.view bIn); cbn; now f_equal. Qed.
 
-    Lemma lookup_insert {b Γ} (bIn : b ∈ Γ) (v : D b) (E : Env (Γ - b)) :
+    Lemma lookup_insert {b Γ} (bIn : b ∈ Γ) (v : D) (E : Env (Γ - b)) :
       lookup (insert bIn E v) bIn = v.
-    Proof. induction Γ; destroy bIn; destroy E; cbn; auto. Qed.
+    Proof. induction bIn; cbn in *. easy. destruct view. cbn. now f_equal. Qed.
 
-    Lemma lookup_thin {b Γ} {E : Env Γ} {bIn : b ∈ Γ} (b' : B) (i : b' ∈ Γ - b) :
-      lookup E (ctx.in_thin bIn i) = lookup (remove b E bIn) i.
+    Lemma lookup_thin {b Γ b'} {E : Env Γ} {bIn : b ∈ Γ} (i : b' ∈ Γ - b) :
+      lookup E (world.in_thin bIn i) = lookup (remove b E bIn) i.
     Proof.
-      induction Γ; destroy bIn; destroy E; destroy i; auto. exact (IHΓ _ _ _).
+      induction bIn; destruct (view E); cbn. easy.
+      destruct (world.view i); cbn; auto.
     Qed.
-
-    Lemma lookup_insert_thin {b Γ} {bIn : b ∈ Γ} {E : Env (Γ - b)}
-      {v : D b} (b' : B) (i : b' ∈ Γ - b) :
-      lookup (insert bIn E v) (ctx.in_thin bIn i) = lookup E i.
-    Proof. now rewrite lookup_thin, remove_insert. Qed.
-
-    (* Slower implementation of insert that is easier to reason about. *)
-    Definition insert' {Γ : Ctx B} {b} (bIn : b ∈ Γ) (E : Env (Γ - b)) (v : D b) : Env Γ :=
-      tabulate (fun x xIn =>
-                  match ctx.occurs_check_view bIn xIn with
-                  | ctx.Same _      => v
-                  | ctx.Diff _ xIn' => lookup E xIn'
-                  end).
-
-    (* Slower implementation of remove that is easier to reason about. *)
-    Definition remove' {Γ b} (E : Env Γ) (bIn : b ∈ Γ) : Env (Γ - b) :=
-      tabulate (fun x xIn => lookup E (ctx.in_thin bIn xIn)).
-    Global Arguments remove' {_} b E.
-
-    Lemma lookup_update_refl {Γ} (E : Env Γ) :
-      forall {b} (bInΓ : b ∈ Γ) (db : D b),
-        lookup (update E bInΓ db) bInΓ = db.
-    Proof.
-      induction E; intros x xIn;
-        destruct (ctx.view xIn); cbn; auto.
-    Qed.
-
-    Lemma lookup_update {eqB : EqDec B} {Γ} (E : Env Γ) :
-      forall (x : B) (xInΓ : x ∈ Γ) (dx : D x) (y : B) (yInΓ : y ∈ Γ),
-        lookup (update E xInΓ dx) yInΓ =
-          match eq_dec (existT x xInΓ) (existT y yInΓ) with
-          | left e => eq_rect x D dx y (f_equal (fun x => projT1 x) e)
-          | right _ => lookup E yInΓ
-          end.
-    Proof.
-      induction E; intros x xIn dx y yIn; destruct (ctx.view xIn), (ctx.view yIn);
-        cbn - [ctx.In_eqdec]; try reflexivity.
-      - rewrite IHE. clear IHE. cbn.  unfold eq_dec.
-        destruct ctx.In_eqdec.
-        + now dependent elimination e.
-        + reflexivity.
-    Qed.
-
-    (* Lemma lookup_update {Γ} (E : Env Γ) : *)
-    (*   forall {b} (bInΓ : b ∈ Γ) (db : D b), *)
-    (*     lookup (update E bInΓ db) bInΓ = db. *)
-    (* Proof. *)
-    (*   induction E; intros ? [n e]; try destruct e; *)
-    (*     destruct n; cbn in *; subst; auto. *)
-    (* Qed. *)
-
-    Lemma drop_cat {Γ Δ} (δΔ : Env Δ) (δΓ : Env Γ) :
-      drop Δ (cat δΓ δΔ) = δΓ.
-    Proof. induction δΔ; cbn; auto. Qed.
-
-    (* Lemma update_update {Γ} (E : Env Γ) : *)
-    (*   forall {b} (bInΓ : b ∈ Γ) (d1 d2 : D b), *)
-    (*     update (update E bInΓ d1) bInΓ d2 = *)
-    (*     update E bInΓ d2. *)
-    (* Proof. *)
-    (*   induction E; intros ? [n e]; [ contradiction e | destruct n ]. *)
-    (*   - destruct e; reflexivity. *)
-    (*   - cbn. intros. f_equal. auto. *)
-    (* Qed. *)
-
-    (* Lemma update_lookup {Γ} (E : Env Γ) : *)
-    (*   forall {b} (bInΓ : b ∈ Γ), *)
-    (*     update E bInΓ (lookup E bInΓ) = E. *)
-    (* Proof. *)
-    (*   induction E; intros ? [n e]; [ contradiction e | destruct n ]. *)
-    (*   - destruct e; reflexivity. *)
-    (*   - cbn. intros. f_equal. auto. *)
-    (* Qed. *)
 
     Lemma lookup_extensional {Γ} (E1 E2 : Env Γ) :
-      (forall {b} (bInΓ : b ∈ Γ), lookup E1 bInΓ = lookup E2 bInΓ) ->
+      (∀ {b} (bInΓ : b ∈ Γ), lookup E1 bInΓ = lookup E2 bInΓ) →
       E1 = E2.
     Proof.
-      induction E1 as [|Γ E1 HE1 b v1]; destroy E2; [easy|].
-      intros Heq. f_equal.
-      - eapply HE1. intros b' bInΓ.
-        apply (Heq b' (ctx.in_succ bInΓ)).
-      - apply (Heq _ ctx.in_zero).
+      induction E1; destruct (view E2); [easy|]. intros Heq. f_equal.
+      - apply IHE1. intros ? bIn. apply (Heq _ (world.in_succ bIn)).
+      - apply (Heq _ world.in_zero).
     Qed.
 
-    Lemma lookup_tabulate {Γ} (g : forall b, b ∈ Γ -> D b) :
-      forall {b} (bInΓ : b ∈ Γ),
-        lookup (tabulate g) bInΓ = g b bInΓ.
-    Proof.
-      induction Γ; intros ? bIn; destroy bIn; [easy|].
-      apply (IHΓ (fun b bInΓ => g b (ctx.in_succ _))).
-    Qed.
-
-    Lemma remove_remove' {Γ x} (E : Env Γ) (xIn : x ∈ Γ) :
-      remove x E xIn = remove' x E xIn.
-    Proof.
-      unfold remove'. induction E; destroy xIn; cbn.
-      - apply lookup_extensional; intros.
-        now rewrite lookup_tabulate.
-      - f_equal. apply IHE.
-    Qed.
-
-    Lemma insert_insert' {Γ x} (xIn : x ∈ Γ) (E : Env (Γ - x)) (v : D x) :
-      insert xIn E v = insert' xIn E v.
-    Proof.
-      unfold insert'. eapply lookup_extensional. intros b' bIn.
-      rewrite lookup_tabulate. destruct ctx.occurs_check_view.
-      - now rewrite lookup_insert.
-      - now rewrite lookup_insert_thin.
-    Qed.
-
-    Lemma lookup_cat_left {Γ1 Γ2 x} (xIn : x ∈ Γ1) (E1 : Env Γ1) (E2 : Env Γ2) :
-      lookup (cat E1 E2) (ctx.in_cat_left Γ2 xIn) = lookup E1 xIn.
-    Proof. induction E2; auto. Qed.
-
-    Lemma lookup_cat_right {Γ1 Γ2 x} (xIn : x ∈ Γ2) (E1 : Env Γ1) (E2 : Env Γ2) :
-      lookup (cat E1 E2) (ctx.in_cat_right xIn) = lookup E2 xIn.
-    Proof. induction E2; destroy xIn; cbn; auto. Qed.
-
-    Fixpoint abstract (Δ : Ctx B) (r : Type) {struct Δ} : Type :=
-      match Δ with
-      | []    => r
-      | Δ ▻ σ => abstract Δ (D σ -> r)
-      end.
-
-    Fixpoint uncurry {Δ : Ctx B} {r : Type} (f : abstract Δ r) (δ : Env Δ) {struct δ} : r :=
-      match δ in Env Δ return forall r : Type, abstract Δ r -> r with
-      | nil       => fun _ v => v
-      | snoc δ db => fun r (f : abstract _ (D _ -> r)) => uncurry f δ db
-      end r f.
-
-    Fixpoint curry {Δ : Ctx B} {r : Type} (f : Env Δ -> r) {struct Δ} : abstract Δ r :=
-      match Δ return forall r : Type, (Env Δ -> r) -> abstract Δ r with
-      | []    => fun r f => f nil
-      | Δ ▻ σ => fun r f => @curry Δ (D σ -> r) (fun E d => f (snoc E d))
-      end r f.
-
-    Fixpoint Forall (Δ : Ctx B) {struct Δ} : (Env Δ -> Prop) -> Prop :=
-      match Δ return (Env Δ -> Prop) -> Prop with
-      | []    => fun P => P nil
-      | Δ ▻ b => fun P => Forall (fun δ => forall v, P (snoc δ v))
-      end.
-
-    Lemma Forall_forall (Δ : Ctx B) (P : Env Δ -> Prop) :
-      (Forall P) <-> (forall E : Env Δ, P E).
-    Proof.
-      split.
-      - induction Δ; intros hyp E; destroy E; [easy|].
-        apply (IHΔ (fun E => forall v, P (snoc E v))).
-        apply hyp.
-      - induction Δ; cbn; [easy|]. intros hyp.
-        now apply (IHΔ (fun E => forall v, P (snoc E v))).
-    Qed.
-
-    Fixpoint Exists (Δ : Ctx B) {struct Δ} : (Env Δ -> Prop) -> Prop :=
-      match Δ return (Env Δ -> Prop) -> Prop with
-      | []    => fun P => P nil
-      | Δ ▻ b => fun P => Exists (fun δ => exists v, P (snoc δ v))
-      end.
-
-    Lemma Exists_exists (Δ : Ctx B) (P : Env Δ -> Prop) :
-      (Exists P) <-> (exists E : Env Δ, P E).
-    Proof.
-      split.
-      - induction Δ; cbn; intros hyp.
-        + now exists nil.
-        + apply IHΔ in hyp. destruct hyp as (E & v & hyp).
-          now exists (snoc E v).
-      - induction Δ; cbn; intros (E & hyp); destroy E; [easy|].
-        apply IHΔ. now exists E, v.
-    Qed.
-
-    Lemma uncurry_curry (Δ : Ctx B) (r : Type) (f : Env Δ -> r) :
-      forall δ, uncurry (curry f) δ = f δ.
-    Proof.
-      intros δ. revert r f.
-      induction δ; cbn; intros; [easy|].
-      now rewrite IHδ.
-    Qed.
-
-    Definition kvsnoc {Γ} (E : Env Γ) (kv : sigT D) : Env (Γ ▻ projT1 kv) :=
-      match kv with
-      | existT k v => @snoc Γ E k v
-      end.
+    Lemma lookup_tabulate {Γ} (g : ∀ b, b ∈ Γ → D) [b] (bIn : b ∈ Γ) :
+      lookup (tabulate g) bIn = g b bIn.
+    Proof. induction bIn; cbn; [easy|apply IHbIn]. Qed.
 
   End WithDom.
 
   Arguments Env : clear implicits.
-  Arguments abstract : clear implicits.
 
   Section Map.
 
-    Context {D1 D2 : B -> Set}.
-    Variable f : forall b, D1 b -> D2 b.
+    Context {D1 D2 : Set} (f : D1 → D2).
 
-    Fixpoint map {Γ} (E : Env D1 Γ) : Env D2 Γ :=
+    Fixpoint map [Γ] (E : Env D1 Γ) : Env D2 Γ :=
       match E with
       | nil       => nil
       | snoc E db => snoc (map E) (f db)
       end.
 
-    Lemma map_cat {Γ1 Γ2} (E1 : Env D1 Γ1) (E2 : Env D1 Γ2) :
-      map (cat E1 E2) = cat (map E1) (map E2).
-    Proof. induction E2; cbn; congruence. Qed.
-
-    Lemma map_drop {Γ Δ} (EΓΔ : Env D1 (Γ ▻▻ Δ)) :
-      map (drop Δ EΓΔ) = drop Δ (map EΓΔ).
-    Proof.
-      induction Δ; intros; cbn in *.
-      - reflexivity.
-      - dependent elimination EΓΔ; apply IHΔ.
-    Qed.
-
-    (* Lemma map_update {Γ} (E : Env D1 Γ) : *)
-    (*   forall {b} (bInΓ : b ∈ Γ) (db : D1 b), *)
-    (*     map (update E bInΓ db) = update (map E) bInΓ (f db). *)
-    (* Proof. *)
-    (*   induction E; intros ? [n e]; try destruct e. *)
-    (*   destruct n; cbn in *; subst; cbn; congruence. *)
-    (* Qed. *)
-
-    Lemma map_tabulate {Γ} (g : forall b, b ∈ Γ -> D1 b) :
-      map (tabulate g) = tabulate (fun b bInΓ => f (g b bInΓ)).
-    Proof.
-      induction Γ; intros; cbn in *.
-      - reflexivity.
-      - f_equal; apply IHΓ.
-    Qed.
-
     Lemma lookup_map {Γ} (E : Env D1 Γ) :
-      forall {b} (bInΓ : b ∈ Γ),
-        lookup (map E) bInΓ = f (lookup E bInΓ).
+      ∀ [b] (bInΓ : b ∈ Γ), lookup (map E) bInΓ = f (lookup E bInΓ).
     Proof.
-      induction E; intros x xIn; destruct (ctx.view xIn); cbn; now subst.
+      induction E; intros x xIn; destruct (world.view xIn); cbn; now subst.
     Qed.
 
   End Map.
 
-  Section WithD123.
-
-    Context {D1 D2 D3 : B -> Set}.
-    Variable f : forall b, D1 b -> D2 b.
-    Variable g : forall b, D2 b -> D3 b.
-
-    Lemma map_map {Γ} (E : Env D1 Γ) :
-      map g (map f E) = map (fun b d => g (f d)) E.
-    Proof. induction E; cbn; f_equal; assumption. Qed.
-
-  End WithD123.
-
-  Lemma map_id_eq {D : B -> Set} {Γ : Ctx B} (f : forall b, D b -> D b) (E : Env D Γ) (hyp_f : forall b d, f b d = d) :
-    map f E = E.
-  Proof. induction E; cbn; congruence. Qed.
-
-  Lemma map_id {D : B -> Set} {Γ : Ctx B} (E : Env D Γ) :
-    map (fun _ d => d) E = E.
-  Proof. now apply map_id_eq. Qed.
-
-  Lemma map_ext {D1 D2 : B -> Set} (f1 f2 : forall b, D1 b -> D2 b) {Γ} (E : Env D1 Γ) :
-    (forall b d, f1 b d = f2 b d) -> map f1 E = map f2 E.
-  Proof.
-    intros HYP.
-    apply lookup_extensional.
-    intros.
-    now rewrite ?lookup_map.
-  Qed.
-
 End WithBinding.
 
-Arguments Env {B} D Γ.
-Arguments nil {B D}.
-Arguments snoc {B%type D%function Γ%ctx} E%env b%ctx & db.
-Arguments lookup {B D Γ} E%env [b] bIn%ctx.
-(* Arguments update {B}%type {D}%function {Γ}%ctx E%env {b}%ctx. *)
-(* Arguments tabulate {_ _} _. *)
-(* Arguments tail {_ _ _} / _. *)
-Arguments abstract {B} D.
-
-Module notations.
-
-  Open Scope dep_pattern_scope.
-  Open Scope env_scope.
-
-  Notation "δ ► ( x ↦ u )" := (snoc δ x u) : env_scope.
-  Notation "δ1 '►►' δ2" := (cat δ1 δ2) : env_scope.
-  (* Notation "δ ⟪ x ↦ v ⟫" := (@update _ _ _ δ (x∷_) _ v) : env_scope. *)
-  (* Based on and compatible with ssrnotations, also used in math-comp finmap.  *)
-  Notation "e .[ i ]" := (@lookup _ _ _ e _ i)
-    (at level 2, left associativity, format "e .[ i ]").
-  (* Based on and compatible with the math-comp finmap notation. *)
-  Notation "e .[? k ]" := (@lookup _ _ _ e k _)
-    (at level 2, k at level 200, format "e .[?  k ]").
-  (* Variant of the above if you don't want to specify the type. *)
-
-  Notation "[ ]" := nil : env_scope.
-  Notation "[ x ]" := (snoc nil _ x) : env_scope.
-  #[deprecated(since="20220204", note="Use the list compatible [ x ; .. ; z ] notation instead.")]
-  Notation "[ x , y , .. , z ]" :=
-    (snoc .. (snoc (snoc nil _ x) _ y) .. _ z)
-    (only parsing) : env_scope.
-  Notation "[ E & x ; y ; .. ; z ]" :=
-    (snoc .. (snoc (snoc E _ x) _ y) .. _ z)
-    (format "[ '['  E  &  x ;  '/' y ;  '/' .. ;  '/' z ']' ]") : env_scope.
-  Notation "[ x ; y ; .. ; z ]" :=
-    (snoc .. (snoc (snoc nil _ x) _ y) .. _ z)
-    (format "[ '[' x ;  '/' y ;  '/' .. ;  '/' z ']' ]") : env_scope.
-  Notation "[ 'env' x ; y ; .. ; z ]" :=
-    (snoc .. (snoc (snoc nil _ x) _ y) .. _ z)
-    (only parsing) : env_scope.
-    (* (format "[ 'env'  '[' x ;  '/' y ;  '/' .. ;  '/' z ']' ]") : env_scope. *)
-
-  (* Sometimes it is necessary to specify both, the element of the context and
-     of the environment in cases where the type-checker would otherwise be
-     blocked on a higher-order unification problem. The list-like notations
-     below allow the user to do so sigma types. *)
-  Notation "[ 'kv' x ]" := (kvsnoc env.nil x)
-    (format "[ 'kv'  x ]") : env_scope.
-  Notation "[ 'kv' x ; y ; .. ; z ]" :=
-    (kvsnoc .. (kvsnoc (kvsnoc env.nil x) y) .. z)
-    (format "[ 'kv'  '[' x ;  '/' y ;  '/' .. ;  '/' z ']' ]") : env_scope.
-
-  (* Notation "'depmatchenv' e 'with' p => rhs 'end'" := *)
-  (*   (match view e with p%dep_pattern => rhs end) *)
-  (*   (at level 0, p pattern, format *)
-  (*    "'[hv' 'depmatchenv'  e  'with'  '/  ' p  =>  '/    ' rhs  '/' 'end' ']'"). *)
-  (* Notation "[ 'env' x ; .. ; z ]" := *)
-  (*   (dsnoc _ .. (dsnoc _ isNil x) .. z) *)
-  (*   (at level 0, format "[ 'env'  x ;  .. ;  z ]") : dep_pattern_scope. *)
-
-End notations.
-
-Local Ltac destroy_env_eq H :=
-  lazymatch type of H with
-  | @eq (Env _ (ctx.snoc _ _)) _ _ =>
-      apply env.inversion_eq_snoc in H;
-      let H1 := fresh in
-      let H2 := fresh in
-      destruct H as [H1 H2];
-      destroy_env_eq H1
-  | @eq (Env _ ctx.nil) env.nil env.nil => clear H
-  | @eq (Env _ ctx.nil) _ _ => idtac
-  end.
+#[global] Arguments Env D w : clear implicits.
+#[global] Arguments nil {D}.
+#[global] Arguments snoc {D w%world} E%env α & d.
 
 Ltac destroy x :=
   try (progress hnf in x);
   lazymatch type of x with
   | Env _ []       => destruct (view x)
   | Env _ (_ ▻ _)  => destruct (view x) as [x]; destroy x
-  | Env _ (_ ▻▻ _) => let E1 := fresh in
-                      let E2 := fresh in
-                      destruct (catView x) as [E1 E2];
-                      destroy E1; destroy E2
-  | _ ∈ []         => destruct (ctx.view x)
-  | _ ∈ _ ▻ _      => destruct (ctx.view x)
-  | @eq ?A ?y ?z   => let A := eval hnf in A in
-                        change_no_check (@eq A y z) in x;
-                        destroy_env_eq x
+  | _ ∈ []         => destruct (world.view x)
+  | _ ∈ _ ▻ _      => destruct (world.view x)
   | _              => idtac
   end.
 
